updated AFP to afp-2014-01-25
Isabelle2013-2

thy_lib/isabelle_afp/Matrix/Matrix_Comparison.thy
@@ -47,7 +47,7 @@ definition vec_comp_all :: "('a \<Rightarrow> 'a \<Rightarrow> bool) \<Rightarro
 
 (* comparison of vectors using >= componentwise *)
 definition vec_ge :: "('a :: non_strict_order) vec \<Rightarrow> 'a vec \<Rightarrow> bool"
-  where "vec_ge \<equiv> vec_comp_all ge"
+  where "vec_ge \<equiv> vec_comp_all (op \<ge>)"
 
 (* comparison of matrices where all components have to be in relation *)
 definition mat_comp_all :: "('a \<Rightarrow> 'a \<Rightarrow> bool) \<Rightarrow> 'a mat \<Rightarrow> 'a mat \<Rightarrow> bool"
@@ -55,7 +55,7 @@ definition mat_comp_all :: "('a \<Rightarrow> 'a \<Rightarrow> bool) \<Rightarro
 
 (* comparison of matrices using >= componentwise *)
 definition mat_ge :: "('a :: non_strict_order) mat \<Rightarrow> 'a mat \<Rightarrow> bool"
-  where "mat_ge \<equiv> mat_comp_all ge"
+  where "mat_ge \<equiv> mat_comp_all (op \<ge>)"
 
 (* demanding at least one strict decrease between two vectors *)
 definition vec_pre_gtI :: "('a \<Rightarrow> 'a \<Rightarrow> bool) \<Rightarrow> 'a vec \<Rightarrow> 'a vec \<Rightarrow> bool"
@@ -77,31 +77,28 @@ definition mat_gtI :: "('a :: non_strict_order \<Rightarrow> 'a \<Rightarrow> bo
 definition mat_monoI :: "('a \<Rightarrow> bool) \<Rightarrow> nat \<Rightarrow> 'a mat \<Rightarrow> bool"
 where "mat_monoI geq1 sd m = Ball (set (sub_mat sd sd m)) (\<lambda> m. Bex (set m) geq1)"
 
-(* max0 on matrices *)
-definition mat_max0 :: "('a :: max_ordered_monoid_add) mat \<Rightarrow> 'a mat"
-  where "mat_max0 \<equiv> mat_map max0"
+(* max on vectors and matrices *)
+abbreviation vec_max where "vec_max \<equiv> vec_plusI (max :: 'a :: ord \<Rightarrow> 'a \<Rightarrow> 'a)"
+abbreviation mat_max where "mat_max \<equiv> mat_plusI (max :: 'a :: ord \<Rightarrow> 'a \<Rightarrow> 'a)"
 
 (* checking whether a matrix is arctic positive (first entry is arctic positive) *)
 definition mat_arc_posI :: "('a \<Rightarrow> bool) \<Rightarrow> 'a mat \<Rightarrow> bool"
 where "mat_arc_posI ap m \<equiv> ap (m ! 0 ! 0)"
 
 (* check whether a matrix is upper triangular *)
-fun upper_triangularI :: "'a \<Rightarrow> 'a \<Rightarrow> ('a \<Rightarrow> 'a \<Rightarrow> bool) \<Rightarrow> 'a mat \<Rightarrow> bool"
-  where "upper_triangularI ze on g [] = True"
-      | "upper_triangularI ze on g ((a # as) # m) = (g on a \<and> (\<forall> b \<in> set as. b = ze) \<and> upper_triangularI ze on g (map tl m))"
-      | "upper_triangularI ze on g ([] # m) = False"
+fun upper_triangular :: "('a :: {ord,one,zero}) mat \<Rightarrow> bool"
+  where "upper_triangular [] = True"
+      | "upper_triangular ((a # as) # m) = (1 \<ge> a \<and> (\<forall> b \<in> set as. b = 0) \<and> upper_triangular (map tl m))"
+      | "upper_triangular ([] # m) = False"
 
 
 subsection {* algorithms preserve dimensions *}
 
-lemma mat_max0: assumes "mat nr nc m" shows "mat nr nc (mat_max0 m)"
-using assms unfolding mat_max0_def by (rule mat_map)
+lemmas mat_max = mat_plus[of _ _ _ _ max]
 
 subsection {* properties of algorithms which do not depend on properties of type of matrix *}
 
-lemma mat_max0_index: assumes wf: "mat nr nc m" and i: "i < nc" and j: "j < nr" 
-  shows "mat_max0 m ! i ! j = max0 (m ! i ! j)"
-unfolding mat_max0_def using assms by (rule mat_map_index)
+lemmas mat_max_index = mat_plus_index[of _ _ _ _ _ _ max]
 
 lemma vec_comp_all_index: assumes "vec nr v1" 
   and "vec nr v2"
@@ -131,19 +128,37 @@ proof (induct nr arbitrary: v1 v2)
   qed
 qed simp
 
-lemma vec_ge_index: assumes "vec nr v1" 
+lemma vec_ge: assumes "vec nr v1" 
   and "vec nr v2"
-  shows "vec_ge v1 v2 = (\<forall> i < nr. ge (v1 ! i) (v2 ! i))"
+  shows "vec_ge v1 v2 = (\<forall> i < nr. (v1 ! i) \<ge> (v2 ! i))"
 using assms
 unfolding vec_ge_def by (rule vec_comp_all_index) 
 
-lemma vec_pre_gt_index: assumes "vec nr v1" 
+lemma vec_geI: assumes wf: "vec nr v1" "vec nr v2"
+  and "\<And> i. i < nr \<Longrightarrow> (v1 ! i) \<ge> (v2 ! i)"
+  shows "vec_ge v1 v2"
+  using assms
+  unfolding vec_ge[OF wf]  by auto 
+
+lemma vec_geE: assumes ge: "vec_ge v1 v2" and wf: "vec nr v1" "vec nr v2"
+  shows "\<And> i. i < nr \<Longrightarrow> (v1 ! i) \<ge> (v2 ! i)"
+  using ge unfolding vec_ge[OF wf] by auto
+
+lemma vec_pre_gt: assumes "vec nr v1" 
   and "vec nr v2"
   shows "vec_pre_gtI gt v1 v2 = (\<exists> i < nr. gt (v1 ! i) (v2 ! i))"
 using assms[simplified vec_def, symmetric]
 by (simp only: Not_eq_iff[symmetric, of "vec_pre_gtI gt v1 v2"], unfold vec_pre_gtI_def, simp add: set_zip, auto) 
+
+lemma vec_pre_gtI: assumes wf: "vec nr v1" "vec nr v2"
+  and "i < nr" "gt (v1 ! i) (v2 ! i)"
+  shows "vec_pre_gtI gt v1 v2" unfolding vec_pre_gt[OF wf] using assms by auto
+
+lemma vec_pre_gtE: assumes gt: "vec_pre_gtI gt v1 v2" and wf: "vec nr v1" "vec nr v2"
+  obtains i where "i < nr" "gt (v1 ! i) (v2 ! i)"
+  using gt unfolding vec_pre_gt[OF wf] by auto
     
-lemma mat_comp_all_index: assumes "mat nr nc m1" 
+lemma mat_comp_all: assumes "mat nr nc m1" 
   and "mat nr nc m2"
   shows "mat_comp_all r m1 m2 = (\<forall> i < nc. \<forall> j < nr. r (m1 ! i ! j) (m2 ! i ! j))"
 using assms
@@ -179,25 +194,39 @@ proof (induct nc arbitrary: m1 m2)
   qed
 qed simp
 
-lemma mat_ge_index: assumes "mat nr nc m1" 
-  and "mat nr nc m2"
-  shows "mat_ge m1 m2 = (\<forall> i < nc. \<forall> j < nr. ge (m1 ! i ! j) (m2 ! i ! j))"
-using assms
-unfolding mat_ge_def by (rule mat_comp_all_index)
+lemma mat_comp_allI: assumes wf: "mat nr nc m1" "mat nr nc m2"
+  and "\<And> i j. i < nc \<Longrightarrow> j < nr \<Longrightarrow> r (m1 ! i ! j) (m2 ! i ! j)"
+  shows "mat_comp_all r m1 m2" unfolding mat_comp_all[OF wf]
+  using assms by auto
 
-lemma mat_pre_gt_index: assumes "mat nr nc m1"
+lemma mat_comp_allE: assumes ge: "mat_comp_all r m1 m2"
+  and wf: "mat nr nc m1" "mat nr nc m2"
+  shows "\<And> i j. i < nc \<Longrightarrow> j < nr \<Longrightarrow> r (m1 ! i ! j) (m2 ! i ! j)"
+  using ge unfolding mat_comp_all[OF wf] by auto
+
+lemma mat_geI: assumes wf: "mat nr nc m1" "mat nr nc m2"
+  and "\<And> i j. i < nc \<Longrightarrow> j < nr \<Longrightarrow> (m1 ! i ! j) \<ge> (m2 ! i ! j)"
+  shows "mat_ge m1 m2" unfolding mat_ge_def 
+  by (rule mat_comp_allI, insert assms, auto)
+
+lemma mat_geE: assumes "mat_ge m1 m2"
+  and "mat nr nc m1" "mat nr nc m2"
+  shows "\<And> i j. i < nc \<Longrightarrow> j < nr \<Longrightarrow> (m1 ! i ! j) \<ge> (m2 ! i ! j)"
+  by (rule mat_comp_allE, insert assms, auto simp: mat_ge_def)
+
+lemma mat_pre_gt: assumes "mat nr nc m1"
   and "mat nr nc m2"
   shows "mat_pre_gtI gt m1 m2 = (\<exists> i < nc. \<exists> j < nr. gt (m1 ! i ! j) (m2 ! i ! j))"
 proof -
   from assms have l1: "nc = length m1" and l2: "length m2 = length m1" 
-    and vl1: "\<forall> i < nc. vec nr (m1 ! i)" and vl2: "\<forall> i < nc. vec nr (m2 ! i)" unfolding mat_def by auto
+    and vl1: "\<And> i. i < nc \<Longrightarrow> vec nr (m1 ! i)" and vl2: "\<And> i. i < nc \<Longrightarrow> vec nr (m2 ! i)" unfolding mat_def by auto
   let ?l = "\<lambda> i. \<not> vec_pre_gtI gt (m1 ! i) (m2 ! i)"
   let ?r = "\<lambda> i. \<forall> j < nr. \<not> gt (m1 ! i ! j) (m2 ! i ! j)"
   have lr: "\<forall> i < nc. ?l i = ?r i"
   proof (intro allI impI)
     fix i
     assume i: "i < nc"
-    show "?l i = ?r i" using vec_pre_gt_index[OF mp[OF spec[OF vl1] i] mp[OF spec[OF vl2] i]] by auto
+    show "?l i = ?r i" using vec_pre_gt[OF vl1[OF i] vl2[OF i]] by auto
   qed     
   show ?thesis
   proof (simp only: Not_eq_iff[symmetric, of "mat_pre_gtI gt m1 m2"], unfold mat_pre_gtI_def set_zip l2 min_max.inf_idem l1[symmetric])
@@ -206,7 +235,15 @@ proof -
   qed
 qed
 
-lemma mat_gt_index: assumes wf1: "mat n n m1"
+lemma mat_pre_gtI: assumes wf: "mat nr nc m1" "mat nr nc m2"
+  and "i < nc" "j < nr" "gt (m1 ! i ! j) (m2 ! i ! j)"
+  shows "mat_pre_gtI gt m1 m2" unfolding mat_pre_gt[OF wf] using assms by auto
+
+lemma mat_pre_gtE: assumes gt: "mat_pre_gtI gt m1 m2" and wf: "mat nr nc m1" "mat nr nc m2"
+  obtains i j where "i < nc" "j < nr" "gt (m1 ! i ! j) (m2 ! i ! j)"
+  using gt unfolding mat_pre_gt[OF wf] by auto
+
+lemma mat_gt: assumes wf1: "mat n n m1"
   and wf2: "mat n n m2"
   and sd: "sd \<le> n"
   shows "mat_gtI gt sd m1 m2 = (mat_ge m1 m2 \<and> (\<exists> i < sd. \<exists> j < sd. gt (m1 ! i ! j) (m2 ! i ! j)))"
@@ -214,14 +251,14 @@ proof -
   have id: "mat_pre_gtI gt (sub_mat sd sd m1) (sub_mat sd sd m2) = (\<exists> i < sd. \<exists> j < sd. gt (m1 ! i ! j) (m2 ! i ! j))" (is "?l = ?r")
   proof -
     have "?l = (\<exists> i < sd. \<exists> j < sd. gt (sub_mat sd sd m1 ! i ! j) (sub_mat sd sd m2 ! i ! j))"
-      by (simp only: mat_pre_gt_index[OF sub_mat[OF wf1 sd sd] sub_mat[OF wf2 sd sd]])
+      by (simp only: mat_pre_gt[OF sub_mat[OF wf1 sd sd] sub_mat[OF wf2 sd sd]])
     also have "\<dots> = ?r" by (simp only: Not_eq_iff[symmetric, of _ ?r], auto simp: sub_mat_index[OF wf1 sd sd] sub_mat_index[OF wf2 sd sd])
     finally show "?l = ?r" .
   qed
   thus ?thesis unfolding mat_gtI_def by auto
 qed
 
-lemma mat_mono_index: assumes wf: "mat n n m"
+lemma mat_mono: assumes wf: "mat n n m"
   and sd: "sd \<le> n" 
   shows "mat_monoI geq1 sd m = (\<forall> i < sd. \<exists> j < sd. geq1 (m ! i ! j))"
 proof -
@@ -266,8 +303,9 @@ proof -
     by auto
 qed
 
+
 lemma upper_triangular: assumes "mat n n m"
-  shows "upper_triangularI ze on g m = (\<forall> i < n. g on (m ! i ! i) \<and> (\<forall> j < n. j > i \<longrightarrow> m ! i ! j = ze))"
+  shows "upper_triangular m = (\<forall> i < n. 1 \<ge> (m ! i ! i) \<and> (\<forall> j < n. j > i \<longrightarrow> m ! i ! j = 0))"
   using assms
 proof (induct n arbitrary: m)
   case 0
@@ -285,10 +323,10 @@ next
   with l have mat: "mat n n ?m" unfolding mat_def by simp
   from v have las: "length as = n" unfolding vec_def by simp
   note IH = Suc(1)[OF mat]
-  let ?l = "\<lambda> i. g on (map tl rs ! i ! i) \<and>
-            (\<forall>j<n. i < j \<longrightarrow> map tl rs ! i ! j = ze)"
-  let ?r = "\<lambda> i. g on (rs ! i ! Suc i) \<and>
-            (\<forall>j<n. i < j \<longrightarrow> rs ! i ! Suc j = ze)"
+  let ?l = "\<lambda> i. 1 \<ge> (map tl rs ! i ! i) \<and>
+            (\<forall>j<n. i < j \<longrightarrow> map tl rs ! i ! j = 0)"
+  let ?r = "\<lambda> i. 1 \<ge> (rs ! i ! Suc i) \<and>
+            (\<forall>j<n. i < j \<longrightarrow> rs ! i ! Suc j = 0)"
   {
     fix i
     assume i: "i < n"
@@ -302,7 +340,7 @@ next
       unfolding rsi by auto      
   }
   hence main: "(\<forall>i<n. ?l i) = (\<forall> i<n. ?r i)" by auto
-  show ?case unfolding m r upper_triangularI.simps
+  show ?case unfolding m r upper_triangular.simps
     unfolding IH 
     unfolding all_Suc_conv
     unfolding all_set_conv_all_nth l las
@@ -320,73 +358,64 @@ lemma mat_ge_refl: "mat_ge m m"
   unfolding mat_ge_def mat_comp_all_def 
   by (induct m, auto simp: vec_ge_refl[unfolded vec_ge_def])
 
-lemma vec_ge_trans: assumes ge12: "vec_ge v1 v2" and ge23: "vec_ge v2 v3" and wf_1: "vec nr v1" and wf_2: "vec nr v2" and wf_3: "vec nr v3"
+lemma vec_ge_trans: assumes ge12: "vec_ge v1 v2" and ge23: "vec_ge v2 v3" and wf: "vec nr v1" "vec nr v2" "vec nr v3"
   shows "vec_ge v1 v3"
-proof (simp only: vec_ge_index[OF wf_1 wf_3], intro allI impI) 
+proof (rule vec_geI)
   fix i
   assume i: "i < nr"
-  show "v1 ! i \<succeq> v3 ! i"
-    using 
-      spec[OF ge12[simplified vec_ge_index[OF wf_1 wf_2]], of i]
-      spec[OF ge23[simplified vec_ge_index[OF wf_2 wf_3]], of i]
-      ge_trans[of "v1 ! i" "v2 ! i" "v3 ! i"]
-      i 
-    by blast
-qed
+  show "v1 ! i \<ge> v3 ! i" using ge_trans[OF vec_geE[OF ge12 _ _ i] vec_geE[OF ge23 _ _ i]] wf by auto
+qed (insert wf, auto)
 
-lemma mat_ge_trans: assumes ge12: "mat_ge v1 v2" and ge23: "mat_ge v2 v3" and wf_1: "mat nr nc v1" and wf_2: "mat nr nc v2" and wf_3: "mat nr nc v3"
+lemma mat_ge_trans: assumes ge12: "mat_ge v1 v2" and ge23: "mat_ge v2 v3" and wf: "mat nr nc v1" "mat nr nc v2" "mat nr nc v3"
   shows "mat_ge v1 v3"
-proof (simp only: mat_ge_index[OF wf_1 wf_3], intro allI impI)
+proof (rule mat_geI)
   fix i j
-  assume i: "i < nc" and j: "j < nr"
-  show "v1 ! i ! j \<succeq> v3 ! i ! j"
-    using 
-      spec[OF ge12[simplified mat_ge_index[OF wf_1 wf_2]], of i]
-      spec[OF ge23[simplified mat_ge_index[OF wf_2 wf_3]], of i]
-      ge_trans[of "v1 ! i ! j" "v2 ! i ! j" "v3 ! i ! j"]
-      i j
-    by blast
-qed
+  assume ij: "i < nc" "j < nr"
+  show "v1 ! i ! j \<ge> v3 ! i ! j" using ge_trans[OF mat_geE[OF ge12 _ _ ij] mat_geE[OF ge23 _ _ ij]] using wf by auto
+qed (insert wf, auto)
 
-lemma vec_plus_left_mono: assumes ge: "vec_ge v1 (v2 :: ('a :: ordered_ab_semigroup)vec)" and wf_1: "vec nr v1" and wf_2: "vec nr v2" and wf_3: "vec nr v3"
+lemma vec_plus_left_mono: assumes ge: "vec_ge v1 (v2 :: ('a :: ordered_ab_semigroup)vec)" and 
+  wf: "vec nr v1" "vec nr v2" "vec nr v3"
   shows "vec_ge (vec_plus v1 v3) (vec_plus v2 v3)"
-  by (simp only: vec_ge_index[OF vec_plus[OF wf_1 wf_3] vec_plus[OF wf_2 wf_3]], intro allI impI,
-    simp only: vec_plus_index[OF wf_1 wf_3],
-    simp only: vec_plus_index[OF wf_2 wf_3],
-    rule plus_left_mono,
-    auto simp: ge[simplified vec_ge_index[OF wf_1 wf_2]])
+proof (rule vec_geI)
+  fix i
+  assume i: "i < nr"
+  note [simp] = vec_plus_index[OF _ _ i] vec_geE[OF ge _ _ i]
+  show "vec_plus v1 v3 ! i \<ge> vec_plus v2 v3 ! i" using wf by (auto intro: plus_left_mono)
+qed (insert wf, auto)
 
-lemma mat_plus_left_mono: assumes ge: "mat_ge m1 (m2 :: ('a :: ordered_ab_semigroup)mat)" and wf_1: "mat nr nc m1" and wf_2: "mat nr nc m2" and wf_3: "mat nr nc m3" 
+lemma mat_plus_left_mono: assumes ge: "mat_ge m1 (m2 :: ('a :: ordered_ab_semigroup)mat)" 
+  and wf: "mat nr nc m1" "mat nr nc m2" "mat nr nc m3" 
   shows "mat_ge (mat_plus m1 m3) (mat_plus m2 m3)"
-by (simp only: mat_ge_index[OF mat_plus[OF wf_1 wf_3] mat_plus[OF wf_2 wf_3]], intro allI impI,
-    simp only: mat_plus_index[OF wf_1 wf_3],
-    simp only: mat_plus_index[OF wf_2 wf_3],
-    rule plus_left_mono,
-    auto simp: ge[simplified mat_ge_index[OF wf_1 wf_2]])
-
+proof (rule mat_geI)
+  fix i j
+  assume i: "i < nc" "j < nr"
+  note [simp] = mat_plus_index[OF _ _ i] mat_geE[OF ge _ _ i]
+  show "mat_plus m1 m3 ! i ! j \<ge> mat_plus m2 m3 ! i ! j" using wf by (auto intro: plus_left_mono)
+qed (insert wf, auto)
 
 lemma scalar_prod_mono_left: assumes wf1: "vec nr (v1 :: ('a :: ordered_semiring_1) vec)"
   and wf2: "vec nr v2"
   and wf3: "vec nr v3"
   and ge1: "vec_ge v1 v2"
   and ge2: "vec_ge v3 (vec0 nr)"
-  shows "scalar_prod v1 v3 \<succeq> scalar_prod v2 v3"
+  shows "scalar_prod v1 v3 \<ge> scalar_prod v2 v3"
 using assms unfolding vec_def vec_ge_def vec_comp_all_def vec0I_def
 proof -
-  assume "length v1 = nr" and "length v2 = nr" and " length v3 = nr" and " \<forall>(x,y)\<in>set (zip v1 v2). x \<succeq> y" and " \<forall>(x,y)\<in>set (zip v3 (replicate nr 0)). x \<succeq> y"
-  thus "scalar_prod v1 v3 \<succeq> scalar_prod v2 v3"
+  assume "length v1 = nr" and "length v2 = nr" and " length v3 = nr" and " \<forall>(x,y)\<in>set (zip v1 v2). x \<ge> y" and " \<forall>(x,y)\<in>set (zip v3 (replicate nr 0)). x \<ge> y"
+  thus "scalar_prod v1 v3 \<ge> scalar_prod v2 v3"
   proof (induct nr arbitrary: v1 v2 v3)
     case (Suc nrr)
     from Suc obtain a1 w1 where v1: "v1 = a1 # w1" and w1: "length w1 = nrr" by (cases v1, auto)
     from Suc obtain a2 w2 where v2: "v2 = a2 # w2" and w2: "length w2 = nrr" by (cases v2, auto)
     from Suc obtain a3 w3 where v3: "v3 = a3 # w3" and w3: "length w3 = nrr" by (cases v3, auto)
-    from Suc have rec: "scalar_prod w1 w3 \<succeq> scalar_prod w2 w3" (is "?l \<succeq> ?r")
+    from Suc have rec: "scalar_prod w1 w3 \<ge> scalar_prod w2 w3" (is "?l \<ge> ?r")
       by (auto simp: w1 w2 w3 v1 v2 v3)
     show ?case proof (simp add: v1 v2 v3 scalar_prod_cons)
-      have one: "a1 * a3 \<succeq> a2 * a3" using times_left_mono[of a3 a1 a2] Suc v1 v2 v3 by auto
-      hence "a1 * a3 + ?l \<succeq> a2 * a3 + ?l" by (rule plus_left_mono)
-      also have "\<dots> \<succeq> a2 * a3 + ?r" using rec by (rule plus_right_mono)
-      finally show "a1 * a3 + ?l \<succeq> a2 * a3 + ?r" .
+      have one: "a1 * a3 \<ge> a2 * a3" using times_left_mono[of a3 a2 a1] Suc v1 v2 v3 by auto
+      hence "a1 * a3 + ?l \<ge> a2 * a3 + ?l" by (rule plus_left_mono)
+      also have "a2 * a3 + ?l \<ge> a2 * a3 + ?r" using rec by (rule plus_right_mono)
+      finally show "a1 * a3 + ?l \<ge> a2 * a3 + ?r" .
     qed
   qed (simp add: scalar_prodI_def ge_refl)
 qed
@@ -396,23 +425,25 @@ lemma scalar_prod_mono_right: assumes wf1: "vec nr (v1 :: ('a :: ordered_semirin
   and wf3: "vec nr v3"
   and ge1: "vec_ge v2 v3"
   and ge2: "vec_ge v1 (vec0 nr)"
-  shows "scalar_prod v1 v2 \<succeq> scalar_prod v1 v3"
+  shows "scalar_prod v1 v2 \<ge> scalar_prod v1 v3"
 using assms unfolding vec_def vec_ge_def vec0I_def vec_comp_all_def
 proof -
-  assume "length v1 = nr" and "length v2 = nr" and " length v3 = nr" and " \<forall>(x,y)\<in>set (zip v2 v3). ge x y" and " \<forall>(x,y)\<in>set (zip v1 (replicate nr 0)). ge x y"
-  thus "ge (scalar_prod v1 v2) (scalar_prod v1 v3)"
+  assume "length v1 = nr" and "length v2 = nr" and " length v3 = nr" 
+    and " \<forall>(x,y)\<in>set (zip v2 v3). x \<ge> y" 
+    and " \<forall>(x,y)\<in>set (zip v1 (replicate nr 0)). x \<ge> y"
+  thus "(scalar_prod v1 v2) \<ge> (scalar_prod v1 v3)"
   proof (induct nr arbitrary: v1 v2 v3)
     case (Suc nrr)
     from Suc obtain a1 w1 where v1: "v1 = a1 # w1" and w1: "length w1 = nrr" by (cases v1, auto)
     from Suc obtain a2 w2 where v2: "v2 = a2 # w2" and w2: "length w2 = nrr" by (cases v2, auto)
     from Suc obtain a3 w3 where v3: "v3 = a3 # w3" and w3: "length w3 = nrr" by (cases v3, auto)
-    from Suc have rec: "scalar_prod w1 w2 \<succeq> scalar_prod w1 w3" (is "?l \<succeq> ?r")
+    from Suc have rec: "scalar_prod w1 w2 \<ge> scalar_prod w1 w3" (is "?l \<ge> ?r")
       by (auto simp: w1 w2 w3 v1 v2 v3)
     show ?case proof (simp add: v1 v2 v3 scalar_prod_cons)
-      have one: "a1 * a2 \<succeq> a1 * a3" using times_right_mono[of a1 a2 a3] Suc v1 v2 v3 by auto
-      hence "a1 * a2 + ?l \<succeq> a1 * a3 + ?l" by (rule plus_left_mono)
-      also have " \<dots> \<succeq> a1 * a3 + ?r" using rec by (rule plus_right_mono)
-      finally show "a1 * a2 + ?l \<succeq> a1 * a3 + ?r" .
+      have one: "a1 * a2 \<ge> a1 * a3" using times_right_mono[of a1 a3 a2] Suc v1 v2 v3 by auto
+      hence "a1 * a2 + ?l \<ge> a1 * a3 + ?l" by (rule plus_left_mono)
+      also have "a1 * a3 + ?l \<ge> a1 * a3 + ?r" using rec by (rule plus_right_mono)
+      finally show "a1 * a2 + ?l \<ge> a1 * a3 + ?r" .
     qed
   qed (simp add: scalar_prodI_def ge_refl)
 qed
@@ -431,23 +462,23 @@ proof -
   from mat_mult[OF wf1 wf3] have wf13: "mat nr ncc ?m13" .
   from mat_mult[OF wf2 wf3] have wf23: "mat nr ncc ?m23" .
   show ?thesis 
-  proof (simp only: mat_ge_index[OF wf13 wf23], intro allI impI)
+  proof (rule mat_geI)
     fix i j
     assume i: "i < ncc" and j: "j < nr"
-    from ge1 have ge1a: "\<forall>i<nc. \<forall> j < nr.  m1 ! i ! j \<succeq> m2 ! i ! j"
-      using mat_ge_index[OF wf1 wf2] by simp
-    from ge2 have ge2a: "\<forall>ia<nc. col m3 i ! ia \<succeq> vec0 nc ! ia"
-      using mat_ge_index[OF wf3 mat0] i unfolding col_def mat0I_def vec0I_def
+    have ge1a: "\<forall>i<nc. \<forall> j < nr.  m1 ! i ! j \<ge> m2 ! i ! j"
+      using mat_geE[OF ge1 wf1 wf2] by simp
+    have ge2a: "\<forall>ia<nc. col m3 i ! ia \<ge> vec0 nc ! ia"
+      using mat_geE[OF ge2 wf3 mat0] i unfolding col_def mat0I_def vec0I_def
       by auto      
-    show "?m13 ! i ! j \<succeq> ?m23 ! i ! j"
-      by (simp only: mat_mult_index[OF wf1 wf3 j i],
-        simp only: mat_mult_index[OF wf2 wf3 j i], 
+    show "?m13 ! i ! j \<ge> ?m23 ! i ! j"
+      by (unfold mat_mult_index[OF wf1 wf3 j i]
+           mat_mult_index[OF wf2 wf3 j i], 
         rule scalar_prod_mono_left[OF row[OF wf1 j] row[OF wf2 j] col[OF wf3 i]],
-        simp only: vec_ge_index[OF row[OF wf1 j] row[OF wf2 j]],
+        unfold vec_ge[OF row[OF wf1 j] row[OF wf2 j]],
         (auto simp: row_col[OF wf1 j] row_col[OF wf2 j] col_def ge1a j)[1],
-        simp only: vec_ge_index[OF col[OF wf3 i] vec0],
+        unfold vec_ge[OF col[OF wf3 i] vec0],
         rule ge2a)
-  qed
+  qed (insert wf1 wf2 wf3, auto)
 qed  
 
 
@@ -464,81 +495,78 @@ proof -
   from mat_mult[OF wf1 wf2] have wf12: "mat nr ncc ?m12" .
   from mat_mult[OF wf1 wf3] have wf13: "mat nr ncc ?m13" .
   show ?thesis 
-  proof (simp only: mat_ge_index[OF wf12 wf13], intro allI impI)
+  proof (rule mat_geI)
     fix i j
     assume i: "i < ncc" and j: "j < nr"
-    from ge2 i have ge2a: " \<forall>ia<nc. col m2 i ! ia \<succeq> col m3 i ! ia"
-      using mat_ge_index[OF wf2 wf3] unfolding col_def by auto
-    from ge1 j have ge1a: " \<forall>i<nc. m1 ! i ! j \<succeq> 0" 
-      using mat_ge_index[OF wf1 mat0] unfolding mat0I_def vec0I_def
+    have ge2a: " \<forall>ia<nc. col m2 i ! ia \<ge> col m3 i ! ia"
+      using mat_geE[OF ge2 wf2 wf3 i] unfolding col_def by auto
+    have ge1a: " \<forall>i<nc. m1 ! i ! j \<ge> 0" 
+      using mat_geE[OF ge1 wf1 mat0] j unfolding mat0I_def vec0I_def
       by auto
-    show "?m12 ! i ! j \<succeq> ?m13 ! i ! j"
-      by  (simp only: mat_mult_index[OF wf1 wf2 j i],
-        simp only: mat_mult_index[OF wf1 wf3 j i],
+    show "?m12 ! i ! j \<ge> ?m13 ! i ! j"
+      by  (unfold mat_mult_index[OF wf1 wf2 j i]
+             mat_mult_index[OF wf1 wf3 j i],
         rule scalar_prod_mono_right[OF row[OF wf1 j] col[OF wf2 i] col[OF wf3 i]], 
-        simp only: vec_ge_index[OF col[OF wf2 i] col[OF wf3 i]], rule ge2a, 
-        simp only: vec_ge_index[OF row[OF wf1 j] vec0],
+        unfold vec_ge[OF col[OF wf2 i] col[OF wf3 i]], rule ge2a, 
+        unfold vec_ge[OF row[OF wf1 j] vec0],
         simp add: row_col[OF wf1 j] vec0I_def col_def, rule ge1a) 
-  qed
+  qed (insert wf1 wf2 wf3, auto)
 qed
 
 lemma mat1_ge_mat0: "mat_ge (mat1 n) ((mat0 n n) :: ('a :: ordered_semiring_1) mat)" (is "mat_ge ?m1 ?m0")
-unfolding mat_ge_index[OF mat1 mat0]
-proof (intro allI impI)
+proof (rule mat_geI)
   fix i j
   assume i: "i < n" and j: "j < n"
   have zero_ij: "?m0 ! i ! j = 0" by (rule mat0_index[OF i j])
   have one_ij: "?m1 ! i ! j = (if i = j then 1 else 0)" by (rule mat1_index[OF i j])
-  show "?m1 ! i ! j \<succeq> ?m0 ! i ! j"
+  show "?m1 ! i ! j \<ge> ?m0 ! i ! j"
     by (simp add: zero_ij one_ij ge_refl one_ge_zero)
-qed
+qed auto
 
-lemma mat_max0_x: assumes wf: "mat nr nc m" shows "mat_ge (mat_max0 m) m"
-proof (unfold mat_ge_index[OF mat_max0[OF wf] wf], intro allI impI)
+lemma mat_max_comm: assumes wf: "mat nr nc m1" "mat nr nc (m2 :: ('a :: non_strict_order) mat)" shows "mat_max m1 m2 = mat_max m2 m1"
+proof (rule mat_eqI)
   fix i j
   assume i: "i < nc" and j: "j < nr"
-  show "mat_max0 m ! i ! j \<succeq> m ! i ! j"
-    by (unfold mat_max0_index[OF wf i j], rule max0_x)
-qed
+  show "mat_max m1 m2 ! i ! j = mat_max m2 m1 ! i ! j"
+    by (unfold mat_max_index[OF wf i j] mat_max_index[OF wf(2,1) i j], rule max_comm)
+qed (insert wf, auto)
 
-lemma mat_max0_pos: assumes wf: "mat nr nc m"
-  shows "mat_ge (mat_max0 m) (mat0 nr nc)"
-proof (unfold mat_ge_index[OF mat_max0[OF wf] mat0], intro allI impI)
+lemma mat_max_ge_x: assumes wf: "mat nr nc m1" "mat nr nc m2" shows "mat_ge (mat_max m1 m2) m1"
+proof (rule mat_geI)
   fix i j
   assume i: "i < nc" and j: "j < nr"
-  show "mat_max0 m ! i ! j \<succeq> mat0 nr nc ! i ! j"
-    by (unfold mat_max0_index[OF wf i j] mat0_index[OF i j], rule max0_pos)
-qed
+  show "mat_max m1 m2 ! i ! j \<ge> m1 ! i ! j"
+    by (unfold mat_max_index[OF wf i j], rule max_ge_x)
+qed (insert wf, auto)
 
-lemma mat_max0_id_pos: assumes ge: "mat_ge m (mat0 nr nc)" and wf: "mat nr nc m"  
-  shows "mat_max0 m = m"
-proof (unfold mat_eq_index[OF mat_max0[OF wf] wf], intro allI impI)
+lemma mat_max_ge: assumes wf1: "mat nr nc m1" and wf2: "mat nr nc m2" 
+  shows "mat_ge (mat_max m1 m2) m1" "mat_ge (mat_max m1 m2) m2"
+  using mat_max_ge_x[OF wf1 wf2] mat_max_ge_x[OF wf2 wf1] unfolding mat_max_comm[OF wf2 wf1]
+  by auto
+
+lemma mat_max_id: assumes ge: "mat_ge m1 m2" and wf: "mat nr nc m1" "mat nr nc m2"
+  shows "mat_max m1 m2 = m1"
+proof (rule mat_eqI)
   fix i j
   assume i: "i < nc" and j: "j < nr"
-  with ge[simplified mat_ge_index[OF wf mat0]] 
-  have "m ! i ! j \<succeq> mat0 nr nc ! i ! j" by simp
-  hence "m ! i ! j \<succeq> 0" using mat0_index[OF i j, of "0 :: 'a"] by simp
-  thus "mat_max0 m ! i ! j = m ! i ! j"
-    by (unfold mat_max0_index[OF wf i j], rule max0_id_pos)
-qed
+  from mat_geE[OF ge _ _ this]
+  have "m1 ! i ! j \<ge> m2 ! i ! j" using wf by auto
+  thus "mat_max m1 m2 ! i ! j = m1 ! i ! j"
+    by (unfold mat_max_index[OF wf i j], rule max_id)
+qed (insert wf, auto)
 
-lemma mat_max0_mono: assumes ge: "mat_ge m1 m2" and wf1: "mat nr nc m1" and wf2: "mat nr nc m2"
-  shows "mat_ge (mat_max0 m1) (mat_max0 m2)"
-proof (unfold mat_ge_index[OF mat_max0[OF wf1] mat_max0[OF wf2]], intro allI impI)
+lemma mat_max_mono: assumes ge: "mat_ge m1 m2" and wf1: "mat nr nc m1" and wf2: "mat nr nc m2"
+  and wf3: "mat nr nc m3"
+  shows "mat_ge (mat_max m3 m1) (mat_max m3 m2)"
+proof (rule mat_geI)
   fix i j
   assume i: "i < nc" and j: "j < nr"
-  with ge[simplified mat_ge_index[OF wf1 wf2]] 
-  have "m1 ! i ! j \<succeq> m2 ! i ! j" by simp
-  hence "max0 (m1 ! i ! j) \<succeq> max0 (m2 ! i ! j)" by (rule max0_mono)
-  thus "mat_max0 m1 ! i ! j \<succeq> mat_max0 m2 ! i ! j"
-    by (unfold mat_max0_index[OF wf1 i j] mat_max0_index[OF wf2 i j])
-qed
-
-context ordered_semiring_1
-begin
-abbreviation upper_triangular where "upper_triangular \<equiv> upper_triangularI (0 :: 'a) 1 ge
-"
-end
+  from mat_geE[OF ge _ _ this] 
+  have "m1 ! i ! j \<ge> m2 ! i ! j" using wf1 wf2 by simp
+  hence "max (m3 ! i ! j) (m1 ! i ! j) \<ge> max (m3 ! i ! j) (m2 ! i ! j)" by (rule max_mono)
+  thus "mat_max m3 m1 ! i ! j \<ge> mat_max m3 m2 ! i ! j"
+    by (unfold mat_max_index[OF wf3 wf1 i j] mat_max_index[OF wf3 wf2 i j])
+qed (insert wf1 wf2 wf3, auto)
 
 lemma mat_pow_ge_zero: assumes m: "mat n n (m :: ('a :: ordered_semiring_1) mat)" and m0: "mat_ge m (mat0 n n)"
   shows "mat_ge (mat_pow n m nn) (mat0 n n)"
@@ -552,16 +580,16 @@ next
     by (rule mat_ge_trans[OF mat_mult_left_mono[OF mat_pow[OF m] mat0 m Suc m0] _ mat_mult[OF mat_pow[OF m] m] mat_mult[OF mat0 m] mat0], unfold mat0_mult_left[OF m], rule mat_ge_refl) 
 qed    
 
-lemma upper_triangular_mat_pow_main: assumes mat: "mat d d (m :: ('a :: {comm_semiring_1, ordered_semiring_1}) mat)"
+lemma upper_triangular_mat_pow_main: assumes mat: "mat d d (m :: ('a :: poly_carrier) mat)"
   and tri: "upper_triangular m"
-  and a: "\<And> i j. i < d \<Longrightarrow> j < d \<Longrightarrow> ge (m ! i ! j) 0 \<and> ge a (m ! i ! j)"
-  and a1: "ge a 1"
-  shows "\<forall> i < d. \<forall> j < d. (i > j \<longrightarrow> mat_pow d m n ! j ! i = 0) \<and> ge (of_nat (fact (j - i)) * (of_nat n * a)^(j - i)) (mat_pow d m n ! j ! i)"
+  and a: "\<And> i j. i < d \<Longrightarrow> j < d \<Longrightarrow> (m ! i ! j) \<ge> 0 \<and> a \<ge> (m ! i ! j)"
+  and a1: "a \<ge> 1"
+  shows "\<forall> i < d. \<forall> j < d. (i > j \<longrightarrow> mat_pow d m n ! j ! i = 0) \<and> (of_nat (fact (j - i)) * (of_nat n * a)^(j - i)) \<ge> (mat_pow d m n ! j ! i)"
 proof -
   let ?n = "of_nat :: nat \<Rightarrow> 'a"
   let ?m = "mat_pow d m"
   let ?p = "\<lambda> n i j. i > j \<longrightarrow> ?m n ! j ! i = 0"
-  let ?q = "\<lambda> n i j. ge (?n (fact (j - i)) * (?n n * a)^(j - i)) (?m n ! j ! i)"
+  let ?q = "\<lambda> n i j. (?n (fact (j - i)) * (?n n * a)^(j - i)) \<ge> (?m n ! j ! i)"
   show "\<forall> i < d. \<forall> j < d. ?p n i j \<and> ?q n i j"
   proof (induct n)
     case 0
@@ -637,8 +665,8 @@ proof -
           by (induct z, auto)
       } note lower_part = this
       hence p: "?p (Suc n) i j" unfolding id by simp
-      from a[OF i i] have a0: "a \<succeq> 0" using ge_trans[of a "m ! i ! i" 0] by auto
-      have na: "\<And> n. ?n n * a \<succeq> (0 :: 'a)"
+      from a[OF i i] have a0: "a \<ge> 0" using ge_trans[of "m ! i ! i" a 0] by auto
+      have na: "\<And> n. ?n n * a \<ge> (0 :: 'a)"
         by (rule mult_ge_zero[OF of_nat_ge_zero a0])
       have "?q (Suc n) i j"
       proof (cases "j < i") 
@@ -703,7 +731,7 @@ proof -
           by (rule nth_map_conv, auto)     
         also have "listsum (?map @ [?fact j]) = listsum ?map + ?fact j" by simp
         finally have sprod: "scalar_prod ?mind ?mcola = listsum ?map + ?fact j" .
-        have "?fsn \<succeq> scalar_prod ?mind ?mcola" 
+        have "?fsn \<ge> scalar_prod ?mind ?mcola" (is "_ \<ge> ?z")
           unfolding sprod
           unfolding diff
           unfolding of_nat_Suc
@@ -719,11 +747,11 @@ proof -
             show ?thesis unfolding 0 by (auto simp: ge_refl field_simps)
           next
             case (Suc dd)                        
-            have ana0: "(1 + ?n n) * a \<succeq> 0"
+            have ana0: "(1 + ?n n) * a \<ge> 0"
               unfolding of_nat_Suc[symmetric] by (rule na)
-            have anana: "(1 + ?n n) * a \<succeq> ?n n * a"
+            have anana: "(1 + ?n n) * a \<ge> ?n n * a"
               using plus_right_mono[OF a0, of "a * ?n n"] by (auto simp: field_simps)
-            have ananapow: "((1 + ?n n) * a) ^ d \<succeq> (?n n * a) ^ d \<and> (?n n * a)^d \<succeq> 0"
+            have ananapow: "((1 + ?n n) * a) ^ d \<ge> (?n n * a) ^ d \<and> (?n n * a)^d \<ge> 0"
               by (rule pow_mono[OF anana na])
             have "?n (fact (Suc d)) * (a + ?n n * a) ^ Suc d = 
               ?n (fact (Suc d)) * ((a + ?n n * a) * (a + ?n n * a) ^ d)" 
@@ -732,72 +760,70 @@ proof -
               ?n (d * fact d) * (a * (a + ?n n * a) ^ d) + 
               ?n (fact d) * (a * (a + ?n n * a) ^ d)" 
               by (simp add: field_simps)
-            also have "... \<succeq> ?n (fact (Suc d)) * ((?n n * a) * (a + ?n n * a) ^ d) + 
+            also have "... \<ge> ?n (fact (Suc d)) * ((?n n * a) * (a + ?n n * a) ^ d) + 
               ?n (d * fact d) * (a * (a + ?n n * a) ^ d) + 
               ?n (fact d) * (1 * (a + ?n n * a) ^ d)" 
               by (rule plus_right_mono[OF times_right_mono[OF of_nat_ge_zero times_left_mono[OF pow_ge_zero a1]]], insert na[of "Suc n"], auto simp: field_simps)
             also have "?n (fact d) * (1 * (a + ?n n * a) ^ d) = ?n (fact d) * (((1 + ?n n) * a) ^ d)" by (simp add: field_simps)
             also have "?n (fact (Suc d)) * ((?n n * a) * (a + ?n n * a) ^ d) + 
               ?n (d * fact d) * (a * (a + ?n n * a) ^ d) + 
-              ?n (fact d) * (((1 + ?n n) * a) ^ d) \<succeq> 
+              ?n (fact d) * (((1 + ?n n) * a) ^ d) \<ge> 
               ?n (fact (Suc d)) * ((?n n * a) * (a + ?n n * a) ^ d) + 
               ?n (d * fact d) * (a * (a + ?n n * a) ^ d) + 
               ((\<Sum>k\<leftarrow>[0..<d]. ?n (fact k) * (?n n * a) ^ k * a) +
-  ?n (fact d) * (?n n * a) ^ d)"
+  ?n (fact d) * (?n n * a) ^ d)" (is "_ \<ge> ?z")
               by (rule plus_right_mono[OF IH])
-            also have "... = ?n (fact (Suc d)) * ((?n n * a) * (a + ?n n * a) ^ d) + 
+            also have "?z = ?n (fact (Suc d)) * ((?n n * a) * (a + ?n n * a) ^ d) + 
               ?n (d * fact d) * (a * (a + ?n n * a) ^ d) + 
               (\<Sum>k\<leftarrow>[0..<d]. ?n (fact k) * (?n n * a) ^ k * a) +
                 ?n (fact d) * (?n n * a) ^ d" by (simp add: field_simps)
-            also have "... \<succeq> ?n (fact (Suc d)) * ((?n n * a) * (a + ?n n * a) ^ d) + 
+            also have "... \<ge> ?n (fact (Suc d)) * ((?n n * a) * (a + ?n n * a) ^ d) + 
               ?n (d * fact d) * (a * (a + ?n n * a) ^ d) + 
               (\<Sum>k\<leftarrow>[0..<d]. ?n (fact k) * (?n n * a) ^ k * a) +
-                0"
+                0" (is "_ \<ge> ?z")
               by (rule plus_right_mono[OF mult_ge_zero[OF of_nat_ge_zero]], insert ananapow, auto)
-            also have "... = ?n (fact (Suc d)) * ((?n n * a) * (a + ?n n * a) ^ d) + 
+            also have "?z = ?n (fact (Suc d)) * ((?n n * a) * (a + ?n n * a) ^ d) + 
               (\<Sum>k\<leftarrow>[0..<d]. ?n (fact k) * (?n n * a) ^ k * a) +
               ?n (d * fact d) * (a * (a + ?n n * a) ^ d)" by (simp add: ac_simps)
-            also have "... \<succeq> ?n (fact (Suc d)) * ((?n n * a) * (a + ?n n * a) ^ d) + 
+            also have "... \<ge> ?n (fact (Suc d)) * ((?n n * a) * (a + ?n n * a) ^ d) + 
               (\<Sum>k\<leftarrow>[0..<d]. ?n (fact k) * (?n n * a) ^ k * a) + 
-              ?n (fact d) * (?n n * a) ^ d * a"
+              ?n (fact d) * (?n n * a) ^ d * a" (is "_ \<ge> ?z")
             proof (rule plus_right_mono)
               have "?n (d * fact d) * (a * (a + ?n n * a) ^ d)
                 = ?n (fact d) * (a * (a + ?n n * a) ^ d) + 
                 ?n (dd * fact d) * (a * (a + ?n n * a) ^ d)" unfolding Suc  by (simp add: field_simps)
-              also have "... \<succeq> ?n (fact d) * (a * (a + ?n n * a) ^ d) + 0"
+              also have "... \<ge> ?n (fact d) * (a * (a + ?n n * a) ^ d) + 0" (is "_ \<ge> ?z")
                 by (rule plus_right_mono[OF mult_ge_zero[OF of_nat_ge_zero mult_ge_zero[OF a0]]], insert ana0, auto simp: field_simps)
-              also have "... = (?n (fact d) * (a + ?n n * a) ^ d) * a"
+              also have "?z = (?n (fact d) * (a + ?n n * a) ^ d) * a"
                 by (auto simp: field_simps)
-              also have "... \<succeq> (?n (fact d) * (?n n * a) ^ d) * a"
+              also have "... \<ge> (?n (fact d) * (?n n * a) ^ d) * a"
                 by (rule times_left_mono[OF a0 times_right_mono[OF of_nat_ge_zero]], insert ananapow, auto simp: field_simps)
-              finally show "?n (d * fact d) * (a * (a + ?n n * a) ^ d) \<succeq> (?n (fact d) * (?n n * a) ^ d) * a" .
+              finally show "?n (d * fact d) * (a * (a + ?n n * a) ^ d) \<ge> (?n (fact d) * (?n n * a) ^ d) * a" .
             qed
-            also have "... = (\<Sum>k\<leftarrow>[0..< Suc d]. ?n (fact k) * (?n n * a) ^ k * a) 
+            also have "?z = (\<Sum>k\<leftarrow>[0..< Suc d]. ?n (fact k) * (?n n * a) ^ k * a) 
                + ?n (fact (Suc d)) * ((?n n * a) * (a + ?n n * a) ^ d)"
               by (simp add: field_simps)
-            also have "... \<succeq> (\<Sum>k\<leftarrow>[0..<Suc d]. ?n (fact k) * (?n n * a) ^ k * a) +
+            also have "... \<ge> (\<Sum>k\<leftarrow>[0..<Suc d]. ?n (fact k) * (?n n * a) ^ k * a) +
               ?n (fact (Suc d)) * (?n n * a) ^ Suc d" unfolding power_Suc
               by (rule plus_right_mono[OF times_right_mono[OF of_nat_ge_zero times_right_mono[OF na]]], insert ananapow, auto simp: field_simps)
             finally
-            show "?n (fact (Suc d)) * ((1 + ?n n) * a) ^ Suc d \<succeq>
+            show "?n (fact (Suc d)) * ((1 + ?n n) * a) ^ Suc d \<ge>
               (\<Sum>k\<leftarrow>[0..<Suc d]. ?n (fact k) * (?n n * a) ^ k * a) +
               ?n (fact (Suc d)) * (?n n * a) ^ Suc d" by (simp add: field_simps)
           qed
         qed      
-        also have "... \<succeq> scalar_prod ?mind ?colj"
+        also have "?z \<ge> scalar_prod ?mind ?colj" (is "_ \<ge> ?z")
         proof (rule scalar_prod_mono_right[OF mind cola col])
           show "vec_ge ?mind (vec0 d)"
-            unfolding vec_ge_index[OF mind vec0] using a0
-            by (auto simp: vec0I_def intro: mult_ge_zero ge_refl)
+            unfolding vec_ge[OF mind vec0] using a0
+            by (auto simp: vec0I_def intro: ge_refl)
         next
-          show "vec_ge ?mcola ?colj" 
-            unfolding vec_ge_index[OF cola col] 
-            unfolding col_def 
-          proof (intro allI impI)
+          show "vec_ge ?mcola ?colj"
+          proof (rule vec_geI[OF cola col], unfold col_def)
             fix i
             assume i: "i < d"
             hence id: "?mcola ! i = ?cola i" by auto
-            have "?cola i \<succeq> m ! j ! i"
+            have "?cola i \<ge> m ! j ! i"
             proof (cases "i < j")
               case True
               with a[OF j i] show ?thesis by auto
@@ -814,30 +840,29 @@ proof -
                 with tri[OF j] i show ?thesis by (auto simp: ge_refl)
               qed
             qed
-            thus "?mcola ! i \<succeq> m ! j ! i" unfolding id .
+            thus "?mcola ! i \<ge> m ! j ! i" unfolding id .
           qed
         qed
-        also have "... \<succeq> scalar_prod ?rowi ?colj"
+        also have "?z \<ge> scalar_prod ?rowi ?colj"
         proof (rule scalar_prod_mono_left[OF mind row col])
           show "vec_ge ?colj (vec0 d)" 
-            unfolding vec_ge_index[OF col vec0]
+            unfolding vec_ge[OF col vec0]
             unfolding col_def vec0I_def using a[OF j] by auto
         next
           show "vec_ge ?mind ?rowi"
-            unfolding vec_ge_index[OF mind row]
-          proof (intro allI impI)
+          proof (rule vec_geI[OF mind row])
             fix j
             assume j: "j < d"
             have idr: "?rowi ! j = ?m n ! j ! i" unfolding row_col[OF mat_pow[OF mat] i j] col_def ..
             have idl: "?mind ! j = ?ind j" using j by auto
             note IH = Suc[rule_format, OF i j]
-            have "?ind j \<succeq> ?m n ! j ! i" 
+            have "?ind j \<ge> ?m n ! j ! i" 
               by (cases "j < i", insert IH, auto simp: ge_refl)
-            thus "?mind ! j \<succeq> ?rowi ! j" unfolding idl idr .
+            thus "?mind ! j \<ge> ?rowi ! j" unfolding idl idr .
           qed
         qed
         finally
-        show "?fsn \<succeq> ?m (Suc n) ! j ! i" unfolding id .
+        show "?fsn \<ge> ?m (Suc n) ! j ! i" unfolding id .
       qed
       with p 
       show "?p (Suc n) i j \<and> ?q (Suc n) i j" ..
@@ -845,17 +870,12 @@ proof -
   qed
 qed
 
-abbreviation vec_max where "vec_max \<equiv> vec_plusI (max :: 'a :: max_ordered_ab_semigroup \<Rightarrow> 'a \<Rightarrow> 'a)"
-abbreviation mat_max where "mat_max \<equiv> mat_plusI (max :: 'a :: max_ordered_ab_semigroup \<Rightarrow> 'a \<Rightarrow> 'a)"
 
-lemmas mat_max_index = mat_plus_index[of _ _ _ _ _ _ max]
-lemmas mat_max = mat_plus[of _ _ _ _ max]
-
-definition max_mat where "max_mat m \<equiv> mat_fold max m (0 :: 'a :: max_ordered_ab_semigroup)"
+definition max_mat where "max_mat m \<equiv> mat_fold max m (0 :: 'a :: ordered_ab_semigroup)"
 
 lemma max_mat: assumes m: "mat nr nc m" 
   and i: "i < nc" and j: "j < nr"
-  shows "max_mat m \<succeq> m ! i ! j"
+  shows "max_mat m \<ge> m ! i ! j"
 proof -
   have id: "max_mat m = foldr max (concat m) 0" 
     unfolding max_mat_def mat_fold.simps vec_fold.simps
@@ -868,21 +888,7 @@ proof -
     by (rule foldr_max[OF mij])
 qed
 
-lemma mat_max_ge: assumes m1: "mat nr nc m1" and m2: "mat nr nc m2"
-  shows "mat_ge (mat_max m1 m2) m1" "mat_ge (mat_max m1 m2) m2"
-proof -
-  have m: "mat nr nc (mat_max m1 m2)"
-    by (rule mat_max[OF m1 m2])
-  note ind = mat_max_index[OF m1 m2]
-  show "mat_ge (mat_max m1 m2) m1"
-    unfolding mat_ge_index[OF m m1]
-    using ind by auto
-  show "mat_ge (mat_max m1 m2) m2"
-    unfolding mat_ge_index[OF m m2]
-    using ind by auto
-qed
-
-definition mat_max_list :: "'a mat list \<Rightarrow> 'a mat \<Rightarrow> ('a :: max_ordered_ab_semigroup) mat"
+definition mat_max_list :: "'a mat list \<Rightarrow> 'a mat \<Rightarrow> ('a :: ordered_ab_semigroup) mat"
   where "mat_max_list ms init \<equiv> foldr mat_max ms init"
 
 lemma mat_max_list: assumes init: "mat nr nc init"
@@ -910,10 +916,10 @@ next
 qed
 
 (* upper triangular matrices grow polynomially in the degree (-1) of the matrix *)
-lemma upper_triangular_mat_pow_index: assumes mat: "mat d d (m :: ('a :: bin_max_ordered_semiring_1) mat)"
+lemma upper_triangular_mat_pow_index: assumes mat: "mat d d (m :: ('a :: poly_carrier) mat)"
   and tri: "upper_triangular m"
   and ge0: "mat_ge m (mat0 d d)"
-  shows "\<exists> c. c \<succeq> 0 \<and> (\<forall> n > 0. \<forall> i < d. \<forall> j < d. ge (c * of_nat n ^ (d - Suc 0)) (mat_pow d m n ! i ! j))"
+  shows "\<exists> c. c \<ge> 0 \<and> (\<forall> n > 0. \<forall> i < d. \<forall> j < d. (c * of_nat n ^ (d - Suc 0)) \<ge> (mat_pow d m n ! i ! j))"
 proof -
   let ?n = "of_nat :: nat \<Rightarrow> 'a"
   let ?d = "d - Suc 0"
@@ -923,16 +929,15 @@ proof -
     fix i j
     assume i: "i < d" and j: "j < d"
     from ge_trans[OF _ max_mat[OF mat i j]]
-    have "a \<succeq> m ! i ! j" unfolding a by auto
+    have "a \<ge> m ! i ! j" unfolding a by auto
   } note am = this
-  have a1: "a \<succeq> 1" unfolding a by auto
-  from ge_trans[OF this one_ge_zero] have a0: "a \<succeq> 0" by simp
-  from ge0[unfolded mat_ge_index[OF mat mat0]]
-  have ge0: "\<And> i j. i < d \<Longrightarrow> j < d \<Longrightarrow> m ! i ! j \<succeq> 0"
-    using mat0_index[of _ d _ d "0 :: 'a"] by auto
+  have a1: "a \<ge> 1" unfolding a by auto
+  from ge_trans[OF this one_ge_zero] have a0: "a \<ge> 0" by simp
+  from mat_geE[OF ge0 mat mat0]
+  have ge0: "\<And> i j. i < d \<Longrightarrow> j < d \<Longrightarrow> m ! i ! j \<ge> 0" by auto
   note main = main[OF conjI[OF ge0 am] a1]
   obtain c where c: "c = ?n (fact ?d) * (a ^ ?d)" by auto
-  have c0: "c \<succeq> 0"
+  have c0: "c \<ge> 0"
     unfolding c
     by (rule mult_ge_zero[OF _ pow_ge_zero[OF a0]], auto)
   show ?thesis
@@ -942,29 +947,29 @@ proof -
     let ?ij = "i - j"
     from i have ijd: "?ij \<le> ?d" by auto
     from main[rule_format, OF _ _ _ _ j i]
-    have ge: "?n (fact (i - j)) * ((?n n * a) ^ (i - j)) \<succeq> mat_pow d m n ! i ! j" ..
-    have na: "?n n * a \<succeq> 0" by (rule mult_ge_zero[OF _ a0], auto)
+    have ge: "?n (fact (i - j)) * ((?n n * a) ^ (i - j)) \<ge> mat_pow d m n ! i ! j" ..
+    have na: "?n n * a \<ge> 0" by (rule mult_ge_zero[OF _ a0], auto)
     have fact: "fact ?d \<ge> fact ?ij"
       by (rule fact_mono_nat[OF ijd])
-    have nfact: "?n (fact ?d) \<succeq> ?n (fact ?ij)" 
+    have nfact: "?n (fact ?d) \<ge> ?n (fact ?ij)" 
       by (rule of_nat_mono[OF fact])
     have "?n n ^ ?d * c = ?n n ^ ?d * (?n (fact ?d) * a ^ ?d)"
       unfolding c by auto
     also have "... = ?n (fact ?d) * ((?n n) ^ ?d * a ^ ?d)" by (auto simp: field_simps)
     also have "((?n n) ^ ?d * a ^ ?d) = (?n n * a) ^ ?d"
       unfolding comm_semiring_1_class.normalizing_semiring_rules ..
-    also have "?n (fact ?d) * (?n n * a) ^ ?d \<succeq> ?n (fact ?ij) * (?n n* a) ^ ?d"
+    also have "?n (fact ?d) * (?n n * a) ^ ?d \<ge> ?n (fact ?ij) * (?n n* a) ^ ?d" (is "_ \<ge> ?z")
       by (rule times_left_mono[OF pow_ge_zero[OF mult_ge_zero[OF _ a0]] nfact], auto)
-    also have "... \<succeq> ?n (fact ?ij) * (?n n * a) ^ ?ij"
+    also have "?z \<ge> ?n (fact ?ij) * (?n n * a) ^ ?ij" (is "_ \<ge> ?z")
     proof (rule times_right_mono[OF of_nat_ge_zero pow_mono_exp[OF mult_ge_one[OF _ a1] ijd]]) 
       from n obtain nn where n: "n = Suc nn" by (cases n, auto)
-      have "?n n \<succeq> 1 + 0" unfolding n of_nat_Suc
+      have "?n n \<ge> 1 + 0" unfolding n of_nat_Suc
         by (rule plus_right_mono, auto)
-      thus "?n n \<succeq> 1" by simp
+      thus "?n n \<ge> 1" by simp
     qed
-    also have "... \<succeq> mat_pow d m n ! i ! j" using ge .
+    also have "?z \<ge> mat_pow d m n ! i ! j" using ge .
     finally
-    show "c * (?n n ^ ?d) \<succeq> mat_pow d m n ! i ! j" by (simp add: field_simps)
+    show "c * (?n n ^ ?d) \<ge> mat_pow d m n ! i ! j" by (simp add: field_simps)
   qed
 qed 
 
@@ -975,17 +980,17 @@ definition linear_norm :: "('a :: monoid_add)mat \<Rightarrow> 'a"
 
 lemma vec_ge_listsum: fixes v1 :: "('a :: ordered_semiring_0) vec"
   assumes v1: "vec nr v1" and v2: "vec nr v2" and ge: "vec_ge v1 v2"
-  shows "listsum v1 \<succeq> listsum v2" 
+  shows "listsum v1 \<ge> listsum v2" 
 proof -
   from v1 v2 have len: "length v1 = length v2" "length v2 = nr" unfolding vec_def by auto
   show ?thesis
-    by (rule listsum_ge_mono[OF len(1), unfolded len(2)], insert ge[unfolded vec_ge_index[OF v1 v2]], auto)
+    by (rule listsum_ge_mono[OF len(1), unfolded len(2)], insert vec_geE[OF ge v1 v2], auto)
 qed
 
 lemma linear_norm_ge: fixes m1 :: "('a :: ordered_semiring_0) mat"
   assumes m1: "mat nr nc m1" and m2: "mat nr nc m2"
   and ge: "mat_ge m1 m2" 
-  shows "linear_norm m1 \<succeq> linear_norm m2"
+  shows "linear_norm m1 \<ge> linear_norm m2"
   using assms 
 proof (induct m1 arbitrary: m2 nc)
   case Nil
@@ -997,10 +1002,10 @@ next
   note Cons = Cons[unfolded this]
   from Cons(4) have v12': "vec_ge v1 v2" and m12ge: "mat_ge m1 m2"
     unfolding mat_ge_def mat_comp_all_def vec_ge_def by auto
-  from vec_ge_listsum[OF v1 v2 v12'] have v12: "listsum v1 \<succeq> listsum v2" .
-  from Cons(1)[OF  m1 m2 m12ge] have m12: "linear_norm m1 \<succeq> linear_norm m2" .
+  from vec_ge_listsum[OF v1 v2 v12'] have v12: "listsum v1 \<ge> listsum v2" .
+  from Cons(1)[OF  m1 m2 m12ge] have m12: "linear_norm m1 \<ge> linear_norm m2" .
   from ge_trans[OF plus_left_mono[OF v12] plus_right_mono[OF m12]]
-  have vm12: "linear_norm (v1 # m1) \<succeq> linear_norm (v2 # m2)" unfolding linear_norm_def by simp
+  have vm12: "linear_norm (v1 # m1) \<ge> linear_norm (v2 # m2)" unfolding linear_norm_def by simp
   thus ?case unfolding m2v .
 qed
 
@@ -1016,38 +1021,39 @@ where "mat_gt \<equiv> mat_gtI gt"
 abbreviation mat_default :: "nat \<Rightarrow> 'a mat" 
 where "mat_default n \<equiv> mat1I 0 default n"
 
+lemma mat_gt_imp_mat_ge: "mat_gt sd m1 m2 \<Longrightarrow> mat_ge m1 m2"
+  unfolding mat_gtI_def by auto
 
 lemma mat_default_ge_mat0: "mat_ge (mat_default n) (mat0 n n)"
-unfolding mat_ge_index[OF mat1 mat0]
-proof (intro allI impI)
+proof (rule mat_geI)
   fix i j
   assume i: "i < n" and j: "j < n"
   have zero_ij: "mat0 n n ! i ! j = 0" by (rule mat0_index[OF i j])
   have one_ij: "mat_default n ! i ! j = (if i = j then default else 0)" by (rule mat1_index[OF i j])
-  show "mat_default n ! i ! j \<succeq> mat0 n n ! i ! j"
+  show "mat_default n ! i ! j \<ge> mat0 n n ! i ! j"
     by (simp add: zero_ij one_ij ge_refl default_ge_zero)
-qed
+qed auto
 
 lemma mat_gt_compat: assumes sd_n: "sd \<le> n" and  ge: "mat_ge m1 m2" and gt: "mat_gt sd m2 m3" and wf1: "mat n n m1" and wf2: "mat n n m2" and wf3: "mat n n m3" 
   shows "mat_gt sd m1 m3"
 proof -
-  from gt[simplified mat_gt_index[OF wf2 wf3 sd_n]] obtain i j 
+  from gt[unfolded mat_gt[OF wf2 wf3 sd_n]] obtain i j 
     where i: "i < sd" and j: "j < sd" and gt: "m2 ! i ! j \<succ> m3 ! i ! j" and ge23: "mat_ge m2 m3" by auto 
-  from ge[simplified mat_ge_index[OF wf1 wf2]] i j sd_n have geij: "m1 ! i ! j \<succeq> m2 ! i ! j" by auto
+  from mat_geE[OF ge wf1 wf2] i j sd_n have geij: "m1 ! i ! j \<ge> m2 ! i ! j" by auto
   from mat_ge_trans[OF ge ge23 wf1 wf2 wf3] have ge: "mat_ge m1 m3" .
   with compat[OF geij gt] i j show ?thesis 
-    by (simp only: mat_gt_index[OF wf1 wf3 sd_n], auto)
+    by (auto simp: mat_gt[OF wf1 wf3 sd_n])
 qed
 
 lemma mat_gt_compat2: assumes sd_n: "sd \<le> n" and gt: "mat_gt sd m1 m2" and ge: "mat_ge m2 m3" and wf1: "mat n n m1" and wf2: "mat n n m2" and wf3: "mat n n m3" 
   shows "mat_gt sd m1 m3"
 proof -
-  from gt[simplified mat_gt_index[OF wf1 wf2 sd_n]] obtain i j 
+  from gt[unfolded mat_gt[OF wf1 wf2 sd_n]] obtain i j 
     where i: "i < sd" and j: "j < sd" and gt: "m1 ! i ! j \<succ> m2 ! i ! j" and ge12: "mat_ge m1 m2" by auto 
-  from ge[simplified mat_ge_index[OF wf2 wf3]] i j sd_n have geij: "m2 ! i ! j \<succeq> m3 ! i ! j" by auto
+  from mat_geE[OF ge wf2 wf3] i j sd_n have geij: "m2 ! i ! j \<ge> m3 ! i ! j" by auto
   from mat_ge_trans[OF ge12 ge wf1 wf2 wf3] have ge: "mat_ge m1 m3" .
   with compat2[OF gt geij] i j show ?thesis 
-    by (simp only: mat_gt_index[OF wf1 wf3 sd_n], auto)
+    by (auto simp: mat_gt[OF wf1 wf3 sd_n])
 qed
 
 lemma mat_gt_trans: assumes sd_n: "sd \<le> n" and  gt1: "mat_gt sd m1 m2" and gt2: "mat_gt sd m2 m3" and wf1: "mat n n m1" and wf2: "mat n n m2" and wf3: "mat n n m3" 
@@ -1074,7 +1080,7 @@ proof -
       by (cases snr, (cases av2, auto)+)
     note Cons = Cons[unfolded av2 snr]
     from Cons(2) have v1: "vec nr v1" unfolding d by simp
-    from Cons(4) have a12: "a1 \<succeq> a2" and v12: "vec_ge v1 v2"
+    from Cons(4) have a12: "a1 \<ge> a2" and v12: "vec_ge v1 v2"
       unfolding vec_ge_def vec_comp_all_def by auto
     from Cons(5) obtain sd where "(a1 \<succ> a2) \<or> (vec_pre_gtI op \<succ> (sub_vec sd v1) (sub_vec sd v2))" 
       unfolding vec_pre_gtI_def sub_vec_def by (cases ssd, auto)
@@ -1093,10 +1099,10 @@ qed
 
 lemma linear_norm_gt_main: assumes m1: "mat nr nc m1" and m2: "mat nr nc m2"
   and ge: "mat_ge m1 m2" 
-  shows "linear_norm m1 \<succeq> linear_norm m2 \<and> (mat_pre_gt (sub_mat sd sdc m1) (sub_mat sd sdc m2) \<longrightarrow> linear_norm m1 \<succ> linear_norm m2)"
+  shows "linear_norm m1 \<ge> linear_norm m2 \<and> (mat_pre_gt (sub_mat sd sdc m1) (sub_mat sd sdc m2) \<longrightarrow> linear_norm m1 \<succ> linear_norm m2)"
 proof -
   note d = vec_def
-  from ge m1 m2 show "(linear_norm m1 \<succeq> linear_norm m2) \<and> (mat_pre_gt (sub_mat sd sdc m1) (sub_mat sd sdc m2) \<longrightarrow> linear_norm m1 \<succ> linear_norm m2)"
+  from ge m1 m2 show "(linear_norm m1 \<ge> linear_norm m2) \<and> (mat_pre_gt (sub_mat sd sdc m1) (sub_mat sd sdc m2) \<longrightarrow> linear_norm m1 \<succ> linear_norm m2)"
   proof (induct m1 arbitrary: m2 nc sdc)
     case Nil
     thus ?case unfolding mat_pre_gtI_def sub_mat_def mat_def by (cases m2, (force simp: ge_refl)+)
@@ -1107,10 +1113,10 @@ proof -
     from Cons(2) have v12': "vec_ge v1 v2" and m12ge: "mat_ge m1 m2"
       unfolding mat_ge_def mat_comp_all_def vec_ge_def by auto
     note IH = Cons(1)[OF m12ge m1 m2]
-    from vec_ge_listsum[OF v1 v2 v12'] have v12: "listsum v1 \<succeq> listsum v2" .
-    from IH have m12: "linear_norm m1 \<succeq> linear_norm m2" by simp
+    from vec_ge_listsum[OF v1 v2 v12'] have v12: "listsum v1 \<ge> listsum v2" .
+    from IH have m12: "linear_norm m1 \<ge> linear_norm m2" by simp
     from ge_trans[OF plus_left_mono[OF v12] plus_right_mono[OF m12]]
-    have vm12: "linear_norm (v1 # m1) \<succeq> linear_norm (v2 # m2)" unfolding linear_norm_def by simp
+    have vm12: "linear_norm (v1 # m1) \<ge> linear_norm (v2 # m2)" unfolding linear_norm_def by simp
     show ?case unfolding m2v
     proof (rule conjI[OF vm12], rule impI)
       assume gt: "mat_pre_gt (sub_mat sd ssdc (v1 # m1)) (sub_mat sd ssdc (v2 # m2))"
@@ -1155,7 +1161,7 @@ qed
 lemma linear_norm_ge_0: fixes m :: "('a :: ordered_semiring_0) mat"
   assumes m: "mat nr nc m" 
   and ge: "mat_ge m (mat0 nr nc)" 
-  shows "linear_norm m \<succeq> 0"
+  shows "linear_norm m \<ge> 0"
   using linear_norm_ge[OF m mat0 ge]
   unfolding linear_norm_0 .
 
@@ -1186,8 +1192,8 @@ next
 qed    
 
 lemma linear_norm_index: fixes m :: "('a :: ordered_semiring_1) mat"   
-  assumes bc: "bc \<succeq> 0"
-  shows "mat nr nc m \<Longrightarrow> \<lbrakk>\<And> i j. i < nc \<Longrightarrow> j < nr \<Longrightarrow> bc \<succeq> m ! i ! j\<rbrakk> \<Longrightarrow> of_nat nr * of_nat nc * bc \<succeq> linear_norm m"
+  assumes bc: "bc \<ge> 0"
+  shows "mat nr nc m \<Longrightarrow> \<lbrakk>\<And> i j. i < nc \<Longrightarrow> j < nr \<Longrightarrow> bc \<ge> m ! i ! j\<rbrakk> \<Longrightarrow> of_nat nr * of_nat nc * bc \<ge> linear_norm m"
 proof (induct nc arbitrary: m)
   case 0 thus ?case using bc unfolding mat_def linear_norm_def 
     by (simp add: ge_refl)
@@ -1196,14 +1202,14 @@ next
   from Suc(2) obtain v m where vm: "vm = v # m" 
     and m: "mat nr nc m" and v: "vec nr v" unfolding mat_def  by (cases vm, auto)
   note Suc = Suc[unfolded vm]
-  from Suc(3)[of 0] have bcv: "\<And> j. j < nr \<Longrightarrow> bc \<succeq> v ! j" by simp
+  from Suc(3)[of 0] have bcv: "\<And> j. j < nr \<Longrightarrow> bc \<ge> v ! j" by simp
   {
     fix i 
     assume "i < nc" 
-    with Suc(3)[of "Suc i"] have "\<And> j. j < nr \<Longrightarrow> bc \<succeq> m ! i ! j" by auto
+    with Suc(3)[of "Suc i"] have "\<And> j. j < nr \<Longrightarrow> bc \<ge> m ! i ! j" by auto
   } note bcm = this
-  from Suc(1)[OF m bcm] have IH: "of_nat nr * of_nat nc * bc \<succeq> linear_norm m" by auto
-  from v bcv have v: "of_nat nr * bc \<succeq> listsum v"
+  from Suc(1)[OF m bcm] have IH: "of_nat nr * of_nat nc * bc \<ge> linear_norm m" by auto
+  from v bcv have v: "of_nat nr * bc \<ge> listsum v"
   proof (induct nr arbitrary: v)
     case 0
     thus ?case unfolding vec_def using bc by (auto simp: ge_refl)
@@ -1212,27 +1218,27 @@ next
     from Suc(2) obtain a v where av: "av = a # v" 
       and v: "vec nr v" unfolding vec_def  by (cases av, auto)
     note Suc = Suc[unfolded av]
-    from Suc(3)[of 0] have a: "bc \<succeq> a" by auto
+    from Suc(3)[of 0] have a: "bc \<ge> a" by auto
     {
       fix i
       assume "i < nr"
-      with Suc(3)[of "Suc i"] have "bc \<succeq> v ! i" by auto 
+      with Suc(3)[of "Suc i"] have "bc \<ge> v ! i" by auto 
     } note bcv = this
-    from Suc(1)[OF v bcv] have IH: "of_nat nr * bc \<succeq> listsum v" by auto
+    from Suc(1)[OF v bcv] have IH: "of_nat nr * bc \<ge> listsum v" by auto
     have "of_nat (Suc nr) * bc = bc + of_nat nr * bc" by (simp add: field_simps)
-    also have "... \<succeq> a + listsum v"
+    also have "... \<ge> a + listsum v"
       by (rule ge_trans[OF plus_left_mono[OF a] plus_right_mono[OF IH]])
     finally show ?case unfolding av by simp
   qed
   have "of_nat nr * of_nat (Suc nc) * bc = of_nat nr * bc + of_nat nr * of_nat nc * bc" by (simp add: field_simps)
-  also have "... \<succeq> listsum v + linear_norm m"
+  also have "... \<ge> listsum v + linear_norm m"
     by (rule ge_trans[OF plus_left_mono[OF v] plus_right_mono[OF IH]])
   finally show ?case unfolding vm linear_norm_def by auto
 qed
 
 lemma linear_norm_submultiplicative: fixes m1 :: "('a :: ordered_semiring_1) mat"
   shows "mat_ge m1 (mat0 nr n) \<Longrightarrow> mat_ge m2 (mat0 n nc) \<Longrightarrow> mat nr n m1 \<Longrightarrow> mat n nc m2 \<Longrightarrow>
-  linear_norm m1 * linear_norm m2 \<succeq> linear_norm (mat_mult nr m1 m2)" 
+  linear_norm m1 * linear_norm m2 \<ge> linear_norm (mat_mult nr m1 m2)" 
 proof (induct n arbitrary: m1 m2)
   case 0
   have m2: "\<forall> x \<in> set m2. x = [] \<Longrightarrow> m2 = replicate (length m2) []"
@@ -1281,8 +1287,7 @@ next
     fix m :: "'a mat" and nr nc
     assume m: "mat nr nc m"
     have "m = ?midx m nr nc" 
-      unfolding mat_eq_index[OF m gen] 
-      by auto
+      by (rule mat_eqI[OF m gen], auto)
   } note mat_idx = this
   let ?mni = "[ m1 ! n ! i . i \<leftarrow> [0..<nr]]"
   let ?min = "[ m2 ! i ! n . i \<leftarrow> [0..<nc]]"
@@ -1323,16 +1328,13 @@ next
   {
     fix m :: "'a mat" and nr nc
     assume m: "mat nr nc m" and ge: "mat_ge m (mat0 nr nc)"
-    from ge[unfolded mat_ge_index[OF m mat0] mat0_index]
-    have ge0: "\<And> i j. i < nc \<Longrightarrow> j < nr \<Longrightarrow> m ! i ! j \<succeq> 0" using mat0_index[of _ nc _ nr "0 :: 'a"]
-      by auto
+    from mat_geE[OF ge m]
+    have ge0: "\<And> i j. i < nc \<Longrightarrow> j < nr \<Longrightarrow> m ! i ! j \<ge> 0" by auto
   } note mat_ge = this
   have ii10: "mat_ge ii1 (mat0 nr n)"
-    unfolding mat_ge_index[OF mat_ii1 mat0] using ii1_idx mat_ge[OF m1 m10] mat0_index[of _ n _ nr "0 :: 'a"]
-    by auto
+    by (rule mat_geI[OF mat_ii1], insert ii1_idx mat_ge[OF m1 m10], auto)
   have ii20: "mat_ge ii2 (mat0 n nc)"
-    unfolding mat_ge_index[OF mat_ii2 mat0] using ii2_idx mat_ge[OF m2 m20] mat0_index[of _ nc _ n "0 :: 'a"]
-    by auto
+    by (rule mat_geI[OF mat_ii2], insert ii2_idx mat_ge[OF m2 m20], auto)
   let ?mult = "mat_mult nr m1 m2"
   have m12: "mat nr nc ?mult" by (rule mat_mult[OF m1 m2])
   {
@@ -1363,8 +1365,7 @@ next
   let ?rii = "listsum [m1 ! n ! j * m2 ! i ! n . i \<leftarrow> [0..<nc], j \<leftarrow> [0..<nr]]"
   {
     have mult_mult': "?mult = ?mult'"
-      unfolding mat_eq_index[OF m12 gen[of _ _ scalar']]
-    proof (intro allI impI)
+    proof (rule mat_eqI[OF m12 gen])
       fix i j
       assume i: "i < nc" and j: "j < nr"
       have "?mult ! i ! j = scalar i j"
@@ -1392,8 +1393,8 @@ next
     ?rii" (is "_ = ?zwi + _") unfolding scalar' unfolding listsum_double_concat  ..
     also have "?zwi = ?vmii"
       unfolding linear_norm_def
-    proof (rule arg_cong[where f = "\<lambda> x. listsum (concat x)"], unfold
-      mat_eq_index[OF gen mat_mult[OF mat_ii1 mat_ii2]], intro allI impI)
+    proof (rule arg_cong[where f = "\<lambda> x. listsum (concat x)"], 
+      rule mat_eqI[OF gen mat_mult[OF mat_ii1 mat_ii2]])
       fix i j
       assume i: "i < nc" and j: "j < nr"
       let ?sc = "(\<lambda> i j. scalar_prod (row (ii1) j) (col (ii2) i))"
@@ -1406,24 +1407,24 @@ next
   } note vmult = this
   have "?v m1 * ?v m2 = ?v (ii1) * ?v (ii2) + (?v (ii1) * ?lmin + ?lmni * ?v (ii2) + ?lmni * ?lmin)"
     unfolding vm1 vm2 by (simp add: field_simps)
-  also have "... \<succeq> ?vmii + (?v (ii1) * ?lmin + ?lmni * ?v (ii2) + ?lmni * ?lmin)"
+  also have "... \<ge> ?vmii + (?v (ii1) * ?lmin + ?lmni * ?v (ii2) + ?lmni * ?lmin)" (is "_ \<ge> ?z")
     by (rule plus_left_mono[OF IH[OF ii10 ii20 mat_ii1 mat_ii2]])
-  also have "... \<succeq> ?vmii + ?rii" 
+  also have "?z \<ge> ?vmii + ?rii" (is "_ \<ge> ?z")
   proof (rule plus_right_mono)
-    from linear_norm_ge_0[OF mat_ii1 ii10] have ii10: "linear_norm ii1 \<succeq> 0" .
-    from linear_norm_ge_0[OF mat_ii2 ii20] have ii20: "linear_norm ii2 \<succeq> 0" .
+    from linear_norm_ge_0[OF mat_ii1 ii10] have ii10: "linear_norm ii1 \<ge> 0" .
+    from linear_norm_ge_0[OF mat_ii2 ii20] have ii20: "linear_norm ii2 \<ge> 0" .
     note m10 = mat_ge[OF m1 m10]
     note m20 = mat_ge[OF m2 m20]
-    have lmin0: "?lmin \<succeq> 0"
+    have lmin0: "?lmin \<ge> 0"
       by (rule listsum_ge_0_nth, insert m20, auto)
-    have lmni0: "?lmni \<succeq> 0"
+    have lmni0: "?lmni \<ge> 0"
       by (rule listsum_ge_0_nth, insert m10, auto)
-    have p10: "?v (ii1) * ?lmin \<succeq> 0"
+    have p10: "?v (ii1) * ?lmin \<ge> 0"
       by (rule mult_ge_zero[OF ii10 lmin0])
-    have p20: "?lmni * ?v (ii2) \<succeq> 0"
+    have p20: "?lmni * ?v (ii2) \<ge> 0"
       by (rule mult_ge_zero[OF lmni0 ii20])
     from plus_right_mono[OF ge_trans[OF plus_left_mono[OF p10] plus_right_mono[OF p20]], of "?lmni * ?lmin"]
-    have ge: "?v (ii1) * ?lmin + ?lmni * ?v (ii2) + ?lmni * ?lmin \<succeq> ?lmni * ?lmin"
+    have ge: "?v (ii1) * ?lmin + ?lmni * ?v (ii2) + ?lmni * ?lmin \<ge> ?lmni * ?lmin"
       by (simp add: ac_simps)
     have id: "?lmni * ?lmin = ?rii" 
     proof (induct nc)
@@ -1446,77 +1447,77 @@ next
       finally
       show ?case .
     qed
-    show "?v (ii1) * ?lmin + ?lmni * ?v (ii2) + ?lmni * ?lmin \<succeq> ?rii" 
+    show "?v (ii1) * ?lmin + ?lmni * ?v (ii2) + ?lmni * ?lmin \<ge> ?rii" 
       using ge unfolding id .
   qed
-  also have "... = ?v ?mult" unfolding vmult ..
+  also have "?z = ?v ?mult" unfolding vmult ..
   finally show ?case .
 qed
 
 
 lemma linear_norm_mult_left_ex: assumes m: "mat n n (m :: ('a :: large_ordered_semiring_1) mat)" 
   and m0: "mat_ge m (mat0 n n)" (is "mat_ge m ?m0")
-  shows "\<exists> c. (\<forall> m'. mat n n m' \<longrightarrow> mat_ge m' (mat0 n n) \<longrightarrow> linear_norm m' * (of_nat c) \<succeq> linear_norm (mat_mult n m' m))"
+  shows "\<exists> c. (\<forall> m'. mat n n m' \<longrightarrow> mat_ge m' (mat0 n n) \<longrightarrow> linear_norm m' * (of_nat c) \<ge> linear_norm (mat_mult n m' m))"
 proof -
   let ?c = "linear_norm m"
-  from linear_norm_ge_0[OF m m0] have c0: "?c \<succeq> 0" .
-  from ex_large_of_nat[of ?c] obtain c where c: "of_nat c \<succeq> ?c" by auto
+  from linear_norm_ge_0[OF m m0] have c0: "?c \<ge> 0" .
+  from ex_large_of_nat[of ?c] obtain c where c: "of_nat c \<ge> ?c" by auto
   show ?thesis
   proof (rule exI[of _ c], intro allI impI)
     fix m' :: "'a mat"
     assume m': "mat n n m'" and m'0: "mat_ge m' (mat0 n n)"
     let ?m' = "linear_norm m'"
-    have "?m' * of_nat c \<succeq> ?m' * ?c"
+    have "?m' * of_nat c \<ge> ?m' * ?c" (is "_ \<ge> ?z")
       by (rule times_right_mono[OF linear_norm_ge_0[OF m' m'0] c])
-    also have "... \<succeq> linear_norm (mat_mult n m' m)"
+    also have "?z \<ge> linear_norm (mat_mult n m' m)"
       by (rule linear_norm_submultiplicative[OF m'0 m0 m' m])
-    finally show "linear_norm m' * of_nat c \<succeq> linear_norm (mat_mult n m' m)" .
+    finally show "linear_norm m' * of_nat c \<ge> linear_norm (mat_mult n m' m)" .
   qed
 qed
 
 lemma linear_norm_mult_right_ex: assumes m: "mat n n (m :: ('a :: large_ordered_semiring_1) mat)" 
   and m0: "mat_ge m (mat0 n n)" (is "mat_ge m ?m0")
-  shows "\<exists> c. (\<forall> m'. mat n n m' \<longrightarrow> mat_ge m' (mat0 n n) \<longrightarrow> linear_norm m' * (of_nat c) \<succeq> linear_norm (mat_mult n m m'))"
+  shows "\<exists> c. (\<forall> m'. mat n n m' \<longrightarrow> mat_ge m' (mat0 n n) \<longrightarrow> linear_norm m' * (of_nat c) \<ge> linear_norm (mat_mult n m m'))"
 proof -
   let ?c = "linear_norm m"
-  from linear_norm_ge_0[OF m m0] have c0: "?c \<succeq> 0" .
-  from ex_large_of_nat[of ?c] obtain c where c: "of_nat c \<succeq> ?c" by auto
+  from linear_norm_ge_0[OF m m0] have c0: "?c \<ge> 0" .
+  from ex_large_of_nat[of ?c] obtain c where c: "of_nat c \<ge> ?c" by auto
   show ?thesis
   proof (rule exI[of _ c], intro allI impI)
     fix m' :: "'a mat"
     assume m': "mat n n m'" and m'0: "mat_ge m' (mat0 n n)"
     let ?m' = "linear_norm m'"
-    have "?m' * of_nat c \<succeq> ?m' * ?c"
+    have "?m' * of_nat c \<ge> ?m' * ?c" (is "_ \<ge> ?z")
       by (rule times_right_mono[OF linear_norm_ge_0[OF m' m'0] c])
-    also have "... = ?c * ?m'" by (simp add: ac_simps)
-    also have "... \<succeq> linear_norm (mat_mult n m m')"
+    also have "?z = ?c * ?m'" by (simp add: ac_simps)
+    also have "... \<ge> linear_norm (mat_mult n m m')"
       by (rule linear_norm_submultiplicative[OF m0 m'0 m m'])
-    finally show "linear_norm m' * of_nat c \<succeq> linear_norm (mat_mult n m m')" .
+    finally show "linear_norm m' * of_nat c \<ge> linear_norm (mat_mult n m m')" .
   qed
 qed
 
 
 
-lemma upper_triangular_mat_pow_value: assumes mat: "mat d d (m :: ('a :: bin_max_ordered_semiring_1) mat)"
+lemma upper_triangular_mat_pow_value: assumes mat: "mat d d (m :: ('a :: poly_carrier) mat)"
   and tri: "upper_triangular m"
   and ge0: "mat_ge m (mat0 d d)"
-  shows "\<exists> c. c \<succeq> 0 \<and> (\<forall> n > 0. ge (c * of_nat (n ^ (d - Suc 0))) (linear_norm (mat_pow d m n)))"
+  shows "\<exists> c. c \<ge> 0 \<and> (\<forall> n > 0. (c * of_nat (n ^ (d - Suc 0))) \<ge> (linear_norm (mat_pow d m n)))"
 proof -
   from upper_triangular_mat_pow_index[OF mat tri ge0]
-  obtain c where "c \<succeq> (0\<Colon>'a) \<and>
-         (\<forall>n>0. \<forall>i<d. \<forall>j<d. c * of_nat n ^ (d - Suc 0) \<succeq>
+  obtain c where "c \<ge> (0\<Colon>'a) \<and>
+         (\<forall>n>0. \<forall>i<d. \<forall>j<d. c * of_nat n ^ (d - Suc 0) \<ge>
                             mat_pow d m n ! i ! j)" ..
-  hence c: "(c :: 'a) \<succeq> 0" and ge: "\<And> n i j. n > 0 \<Longrightarrow> i < d \<Longrightarrow> j < d \<Longrightarrow> c * of_nat n ^ (d - Suc 0) \<succeq> mat_pow d m n ! i ! j" by auto
+  hence c: "(c :: 'a) \<ge> 0" and ge: "\<And> n i j. n > 0 \<Longrightarrow> i < d \<Longrightarrow> j < d \<Longrightarrow> c * of_nat n ^ (d - Suc 0) \<ge> mat_pow d m n ! i ! j" by auto
   let ?c = "of_nat d * of_nat d * c"
-  from c have c0: "?c \<succeq> 0" by auto
+  from c have c0: "?c \<ge> 0" by auto
   show ?thesis
   proof (rule exI, rule conjI[OF c0], intro allI impI)
     fix n :: nat
     assume n: "0 < n"
-    hence "?c * of_nat n ^ (d - Suc 0) \<succeq> linear_norm (mat_pow d m n)"
+    hence "?c * of_nat n ^ (d - Suc 0) \<ge> linear_norm (mat_pow d m n)"
       using linear_norm_index[OF _ mat_pow[OF mat] ge[OF n]] c 
       by (auto simp: field_simps)
-    thus "?c * of_nat (n ^ (d - Suc 0)) \<succeq> linear_norm (mat_pow d m n)"
+    thus "?c * of_nat (n ^ (d - Suc 0)) \<ge> linear_norm (mat_pow d m n)"
       unfolding of_nat_power .
   qed
 qed
@@ -1527,24 +1528,25 @@ begin
 lemma mat_plus_gt_left_mono: assumes sd_n: "sd \<le> n" and gt: "mat_gt sd m1 m2" and ge: "mat_ge m3 m4" and wf1: "mat n n m1" and wf2: "mat n n m2" and wf3: "mat n n m3" and wf4: "mat n n m4"
   shows "mat_gt sd (mat_plus m1 m3) (mat_plus m2 m4)"
 proof -
+  note wf = wf1 wf2 wf3 wf4
   let ?m13 = "mat_plus m1 m3"
   let ?m23 = "mat_plus m2 m3"
   let ?m32 = "mat_plus m3 m2"
   let ?m24 = "mat_plus m2 m4"
   let ?m42 = "mat_plus m4 m2"
-  have wf13: "mat n n ?m13" and wf24: "mat n n ?m24" by ((rule mat_plus[of n n], auto simp: wf1 wf2 wf3 wf4)+)
-  from gt[simplified mat_gt_index[OF wf1 wf2 sd_n]] obtain i j where
+  have wf13: "mat n n ?m13" and wf24: "mat n n ?m24" using wf by auto
+  from gt[simplified mat_gt[OF wf1 wf2 sd_n]] obtain i j where
     i: "i < sd" and j: "j < sd" and gt: "m1 ! i ! j \<succ> m2 ! i ! j" and ge12: "mat_ge m1 m2" by auto
   with sd_n have ni: "i < n" and nj: "j < n" by auto
   from mat_plus_left_mono[OF ge12 wf1 wf2 wf3] have one: "mat_ge ?m13 ?m23" .
   from mat_plus_left_mono[OF ge wf3 wf4 wf2] have "mat_ge ?m32 ?m42" .
   hence two: "mat_ge ?m23 ?m24" by (simp add: mat_plus_comm[of m2 m3] mat_plus_comm[of m2 m4])
-  have matge: "mat_ge ?m13 ?m24" by (rule mat_ge_trans[OF one two, of n n], (rule mat_plus[of n n], auto simp: wf1 wf2 wf3 wf4)+)
-  from i j sd_n ge[simplified mat_ge_index[OF wf3 wf4]] have ge: "m3 ! i ! j \<succeq> m4 ! i ! j" by auto
+  have matge: "mat_ge ?m13 ?m24" by (rule mat_ge_trans[OF one two], insert wf, auto)
+  from i j sd_n mat_geE[OF ge] wf have ge: "m3 ! i ! j \<ge> m4 ! i ! j" by auto
   from compat2[OF plus_gt_left_mono[OF gt] plus_right_mono[OF ge]] mat_plus_index[OF wf1 wf3 ni nj] mat_plus_index[OF wf2 wf4 ni nj]      
   have gt: "?m13 ! i ! j \<succ> ?m24 ! i ! j" by simp
   from i j matge gt  show ?thesis 
-    by (auto simp: mat_gt_index[OF wf13 wf24 sd_n] matge)
+    by (auto simp: mat_gt[OF wf13 wf24 sd_n] matge)
 qed
 
 lemma mat_default_gt_mat0: assumes sd_pos: "sd > 0" and sd_n: "sd \<le> n"
@@ -1552,7 +1554,7 @@ lemma mat_default_gt_mat0: assumes sd_pos: "sd > 0" and sd_n: "sd \<le> n"
 proof -
   from assms have n: "n > 0" by auto
   show ?thesis 
-    by (simp only: mat_gt_index[OF mat1 mat0 sd_n] mat_default_ge_mat0, rule conjI[OF TrueI],
+    by (simp only: mat_gt[OF mat1 mat0 sd_n] mat_default_ge_mat0, rule conjI[OF TrueI],
       (rule exI[of _ 0], simp only: sd_pos, rule conjI[OF TrueI])+, simp add: mat1_index[OF n n] mat0_index[OF n n] default_gt_zero)
 qed
 end
@@ -1562,7 +1564,7 @@ text {* three easy lemmas to go from pairs of numbers to numbers  *}
 lemma mul_div_eq: assumes "c < b" shows "(a * b + c) div b = (a :: nat)" 
 proof -
   from assms have b: "b \<noteq> 0" by simp
-  have "(a * b + c) div b = (c + a * b) div b" by arith
+  have "(a * b + c) div b = (c + a * b) div b" by presburger
   also have "\<dots> = c div b + a" using b by simp
   also have "\<dots> = a" using assms by simp
   finally show ?thesis .
@@ -1618,8 +1620,8 @@ qed simp
 context SN_one_mono_ordered_semiring_1
 begin
 
-abbreviation mat_ns :: "'a mat \<Rightarrow> nat \<Rightarrow> 'a mat \<Rightarrow> bool" ("(_ \<succeq>m _ _)" [51,51,51] 50) 
- where "m1 \<succeq>m n m2 \<equiv> (mat n n m1 \<and> mat n n m2 \<and> mat_ge m1 m2)"
+abbreviation mat_ns :: "'a mat \<Rightarrow> nat \<Rightarrow> 'a mat \<Rightarrow> bool" ("(_ \<ge>m _ _)" [51,51,51] 50) 
+ where "m1 \<ge>m n m2 \<equiv> (mat n n m1 \<and> mat n n m2 \<and> mat_ge m1 m2)"
 
 abbreviation mat_s :: "'a mat \<Rightarrow> nat \<Rightarrow> nat \<Rightarrow> 'a mat \<Rightarrow> bool" ("(_ \<succ>m _ _ _)" [51,51,51,51] 50)
  where "m1 \<succ>m n sd m2 \<equiv> (mat n n m1 \<and> mat n n m2 \<and> mat_ge m2 (mat0 n n) \<and> mat_gt sd m1 m2)"
@@ -1627,43 +1629,44 @@ abbreviation mat_s :: "'a mat \<Rightarrow> nat \<Rightarrow> nat \<Rightarrow> 
 lemma mat_sn: assumes sd_n: "sd \<le> n" shows "SN {(m1,m2) . m1 \<succ>m n sd m2}"
 unfolding SN_defs
 proof clarify
-  fix e f 
-  assume ass: "\<forall> i. (f i, f (Suc i)) \<in> {(m1,m2). m1 \<succ>m n sd m2}"
+  fix f 
+  assume "\<forall> i. (f i, f (Suc i)) \<in> {(m1,m2). m1 \<succ>m n sd m2}"
+  hence ass: "\<And> i. (f i, f (Suc i)) \<in> {(m1,m2). m1 \<succ>m n sd m2}" by blast
   hence len_n: "\<And> i. length (f i) = n" by (auto simp: mat_def) 
-  let ?rel = "{(x,y). y \<succeq> 0 \<and> x \<succ> y}"
+  let ?rel = "{(x,y). y \<ge> 0 \<and> x \<succ> y}"
   let ?gt = "\<lambda> k i j. f k ! i ! j \<succ> f (Suc k) ! i ! j"
-  let ?ge = "\<lambda> k i j. f k ! i ! j \<succeq> f (Suc k) ! i ! j"
-  let ?gez = "\<lambda> k i j. f (Suc k) ! i ! j \<succeq> 0"
+  let ?ge = "\<lambda> k i j. f k ! i ! j \<ge> f (Suc k) ! i ! j"
+  let ?gez = "\<lambda> k i j. f (Suc k) ! i ! j \<ge> 0"
   let ?f = "\<lambda> k ij. f k ! (ij div sd) ! (ij mod sd)"
   let ?ij = "\<lambda> i j. (i * sd + j)"
   let ?fgt = "\<lambda> k ij. (?f k ij,?f (Suc k) ij) \<in> ?rel"
   let ?fpgt = "\<lambda> k ij. ?f k ij \<succ> ?f (Suc k) ij"
-  let ?fge = "\<lambda> k ij. ?f k ij \<succeq> ?f (Suc k) ij"
+  let ?fge = "\<lambda> k ij. ?f k ij \<ge> ?f (Suc k) ij"
   let ?sd = "sd * sd"
   have all: "\<And> k. (\<exists> ij < ?sd. ?fgt k ij) \<and> (\<forall> ij < ?sd. ?fge k ij)"
   proof -
     fix k
-    from spec[OF ass, of k] have wf: "mat n n (f k)" and wf1: "mat n n (f (Suc k))" and gt: "mat_gt sd (f k) (f (Suc k))" and
+    from ass[of k] have wf: "mat n n (f k)" and wf1: "mat n n (f (Suc k))" and gt: "mat_gt sd (f k) (f (Suc k))" and
       gez: "mat_ge (f (Suc k)) (mat0 n n)" by auto
-    from gt[simplified mat_gt_index[OF wf wf1 sd_n]] obtain i j where i: "i < sd" and j: "j < sd" and ge: "mat_ge (f k) (f (Suc k))"
+    from gt[simplified mat_gt[OF wf wf1 sd_n]] obtain i j where i: "i < sd" and j: "j < sd" and ge: "mat_ge (f k) (f (Suc k))"
       and gt: "?gt k i j" by auto
     hence pgt: "?fpgt k (?ij i j)" by (auto simp: mul_div_eq[OF j] j)
     have ij: "?ij i j < ?sd" using i j smaller_product by auto
-    from ge[simplified mat_ge_index[OF wf wf1]] sd_n have "\<forall> i < sd. \<forall> j < sd. ?ge k i j" by auto
+    from mat_geE[OF ge wf wf1] sd_n have "\<forall> i < sd. \<forall> j < sd. ?ge k i j" by auto
     hence ge: "\<forall> ij < ?sd. ?fge k ij" by (simp add: all_all_into_all)      
-    from gez[simplified mat_ge_index[OF wf1 mat0]] sd_n have "\<forall> i < sd. \<forall> j < sd. ?gez k i j" by (auto simp: mat0_index)
+    from mat_geE[OF gez wf1 mat0] sd_n have "\<forall> i < sd. \<forall> j < sd. ?gez k i j" by auto
     hence "?gez k i j" using i j by simp
-    hence "?f (Suc k) (?ij i j) \<succeq> 0" by (auto simp: mul_div_eq[OF j] j)
+    hence "?f (Suc k) (?ij i j) \<ge> 0" by (auto simp: mul_div_eq[OF j] j)
     with pgt have gt: "?fgt k (?ij i j)" by auto 
     from gt ge ij show "(\<exists> ij < ?sd. ?fgt k ij) \<and> (\<forall> ij < ?sd. ?fge k ij)" by auto
   qed
   obtain f sd where f: "f = ?f" and "sd = ?sd" by auto
-  with all have ex: "\<And> k. (\<exists> i < sd. (f k i, f (Suc k) i) \<in> ?rel)" and all: "\<And> k.(\<forall> i < sd. f k i \<succeq> f (Suc k) i)" by auto
+  with all have ex: "\<And> k. (\<exists> i < sd. (f k i, f (Suc k) i) \<in> ?rel)" and all: "\<And> k.(\<forall> i < sd. f k i \<ge> f (Suc k) i)" by auto
   let ?g = "\<lambda> k i. (f k i, f (Suc k) i) \<in> ?rel"
   from ex have g: "\<forall> k. \<exists> i < sd. ?g k i" by auto
   from inf_pigeonhole_principle[OF g] obtain i where i: "i < sd" and inf: "\<forall> k. \<exists> k' \<ge> k. ?g k' i" by auto
   let ?h = "\<lambda> k. (f k i)"
-  let ?nRel = "{(x,y) | x y :: 'a. x \<succeq> y}"
+  let ?nRel = "{(x,y) | x y :: 'a. x \<ge> y}"
   from all i have all: "\<forall> k. (?h k, ?h (Suc k)) \<in> ?nRel \<union> ?rel" by auto
   from SN have SNe: "SN_on ?rel {?h 0}" unfolding SN_defs by auto
   have comp: "?nRel O ?rel \<subseteq> ?rel" using compat by auto
@@ -1689,11 +1692,11 @@ proof -
   from wf1 wf3 have wf13: "mat n n ?m13" by (rule mat_mult)
   from mat_mult_right_mono[OF wf1 wf2 wf3 ge] gt have gem: "mat_ge ?m12 ?m13" unfolding mat_gtI_def by auto
   from gt obtain i j where i: "i < sd" and j: "j < sd" and gt: "m2 ! i ! j \<succ> m3 ! i ! j" and geq: "mat_ge m2 m3"
-    by (auto simp: mat_gt_index[OF wf2 wf3 sd_n])
-  from mmono mat_mono_index[OF wf1 sd_n] j obtain k where k: "k < sd" and monojk: "mono (m1 ! j ! k)" by auto
+    by (auto simp: mat_gt[OF wf2 wf3 sd_n])
+  from mmono mat_mono[OF wf1 sd_n] j obtain k where k: "k < sd" and monojk: "mono (m1 ! j ! k)" by auto
   from i j k sd_n have ni: "i < n" and nj: "j < n" and nk: "k < n" by auto
   show ?thesis 
-  proof (simp only: mat_gt_index[OF wf12 wf13 sd_n], simp only: gem, rule conjI[OF TrueI],
+  proof (simp only: mat_gt[OF wf12 wf13 sd_n], simp only: gem, rule conjI[OF TrueI],
       rule exI[of _ i], simp only: i, rule conjI[OF TrueI],
       rule exI[of _ k], simp only: k, rule conjI[OF TrueI])
     let ?r = "\<lambda> n. map (\<lambda> j. m1 ! j ! k) [0 ..< n]"
@@ -1702,30 +1705,30 @@ proof -
     from col[OF wf3 ni] have wfc3: "length (col m3 i) = n" unfolding vec_def by auto
     have "row m1 k = map (\<lambda> i. row m1 k ! i) [0 ..< length (row m1 k)]" by (rule map_nth[symmetric])
     also have "\<dots> = map (\<lambda> i. row m1 k !  i) [0 ..< n]" by (simp add: wfr)
-    also have "\<dots> = ?r n" using row_col[OF wf1 nk, simplified col_def]
+    also have "\<dots> = ?r n" using row_col[OF wf1 nk, unfolded col_def]
       by auto
     finally have r: "row m1 k = ?r n" .
     let ?c2 = "\<lambda> n. map (\<lambda> j. m2 ! i ! j) [0 ..< n]"
-    have c2: "col m2 i = ?c2 n" by (simp only: wfc2[symmetric] col_def, simp add: map_nth)
+    have c2: "col m2 i = ?c2 n" unfolding wfc2[symmetric] col_def by (simp add: map_nth)
     let ?c3 = "\<lambda> n. map (\<lambda> j. m3 ! i ! j) [0 ..< n]"
-    have c3: "col m3 i = ?c3 n" by (simp only: wfc3[symmetric] col_def, simp add: map_nth)
+    have c3: "col m3 i = ?c3 n" unfolding wfc3[symmetric] col_def by (simp add: map_nth)
     from mat_mult_index[OF wf1 wf2 nk ni]
     have s12: "?m12 ! i ! k = scalar_prod (?r n) (?c2 n)" by (simp add: r c2)
     from mat_mult_index[OF wf1 wf3 nk ni]
     have s13: "?m13 ! i ! k = scalar_prod (?r n) (?c3 n)" by (simp add: r c3)
-    have r0: "\<forall> j < n. ?r n ! j \<succeq> 0" 
+    have r0: "\<forall> j < n. ?r n ! j \<ge> 0" 
     proof (intro impI allI)
       fix j
       assume "j < n"
-      with ge[simplified mat_ge_index[OF wf1 mat0]] nk
-      show "?r n ! j \<succeq> 0" by (simp add: mat0_index)
+      with mat_geE[OF ge wf1 mat0] nk
+      show "?r n ! j \<ge> 0" by simp
     qed
-    have c2c3: "\<forall> j < n. ?c2 n ! j \<succeq> ?c3 n ! j"
+    have c2c3: "\<forall> j < n. ?c2 n ! j \<ge> ?c3 n ! j"
     proof (intro impI allI)
       fix j
       assume "j < n"
-      with ni geq[simplified mat_ge_index[OF wf2 wf3]] 
-      show "?c2 n ! j \<succeq> ?c3 n ! j" by simp
+      with ni mat_geE[OF geq wf2 wf3] 
+      show "?c2 n ! j \<ge> ?c3 n ! j" by simp
     qed
     from nj r0 c2c3 have "scalar_prod (?r n) (?c2 n) \<succ> scalar_prod (?r n) (?c3 n)"
     proof (induct n)
@@ -1740,19 +1743,19 @@ proof -
       also have "\<dots> = m1 ! n ! k * m3 ! i ! n + scalar_prod (?r n) (?c3 n)" (is "_ = plus ?p3 ?s3") 
         by (simp add: scalar_prod_last)
       finally have sum3: "?sum3 = ?p3 + ?s3" .
-      from Suc(3) have z: "m1 ! n ! k \<succeq> 0" by (simp del: upt_Suc)
-      from Suc(3) have za: "\<forall> j < n. ?r n ! j \<succeq> 0"  by (simp del: upt_Suc)
-      from Suc(4) have ge: "\<forall> j < n. ?c2 n ! j \<succeq> ?c3 n ! j"  by (simp del: upt_Suc)
+      from Suc(3) have z: "m1 ! n ! k \<ge> 0" by (simp del: upt_Suc)
+      from Suc(3) have za: "\<forall> j < n. ?r n ! j \<ge> 0"  by (simp del: upt_Suc)
+      from Suc(4) have ge: "\<forall> j < n. ?c2 n ! j \<ge> ?c3 n ! j"  by (simp del: upt_Suc)
       show ?case
       proof (cases "j = n")
         case False
         with Suc(2) have j: "j < n" by auto
         have rec: "?s2 \<succ> ?s3"
           by (rule Suc, rule j, rule za, rule ge)
-        from Suc(4) have ge: "m2 ! i ! n \<succeq> m3 ! i ! n" by (simp del: upt_Suc)
-        from times_right_mono[OF z ge] have p23: "?p2 \<succeq> ?p3" .
+        from Suc(4) have ge: "m2 ! i ! n \<ge> m3 ! i ! n" by (simp del: upt_Suc)
+        from times_right_mono[OF z ge] have p23: "?p2 \<ge> ?p3" .
         from compat2[OF plus_gt_left_mono[OF rec] plus_right_mono[OF p23]] have "?s2 + ?p2 \<succ> ?s3 + ?p3" .
-        with add_commute[of ?p2] add_commute[of ?p3] have "?p2 + ?s2 \<succ> ?p3 + ?s3" by simp
+        hence "?p2 + ?s2 \<succ> ?p3 + ?s3" unfolding add_commute[of ?p2] add_commute[of ?p3] .
         with sum2 sum3 show ?thesis by simp 
       next
         case True        
@@ -1760,11 +1763,9 @@ proof -
         have wf1: "vec n (?r n)" by (simp add: vec_def)
         have wf2: "vec n (?c2 n)" by (simp add: vec_def)
         have wf3: "vec n (?c3 n)" by (simp add: vec_def)
-        from ge have ge: "vec_ge (?c2 n) (?c3 n)" 
-          by (simp only: vec_ge_index[OF wf2 wf3])
-        from za have z: "vec_ge (?r n) (vec0 n)" 
-          by (simp only: vec_ge_index[OF wf1 vec0], auto simp: vec0I_def)
-        have s23: "?s2 \<succeq> ?s3"
+        from ge have ge: "vec_ge (?c2 n) (?c3 n)" unfolding vec_ge[OF wf2 wf3] by simp
+        from za have z: "vec_ge (?r n) (vec0 n)" unfolding vec_ge[OF wf1 vec0] by (simp add: vec0I_def)
+        have s23: "?s2 \<ge> ?s3"
           by (rule scalar_prod_mono_right, (simp add: vec_def)+, rule ge, rule z)
         from compat2[OF plus_gt_left_mono[OF p23] plus_right_mono[OF s23]] sum2 sum3 show ?thesis by simp
       qed
@@ -1782,6 +1783,10 @@ where "mat_gt_arc \<equiv> mat_comp_all gt"
 
 abbreviation mat_arc_pos :: "'a mat \<Rightarrow> bool"
 where "mat_arc_pos \<equiv> mat_arc_posI arc_pos"
+
+lemma mat_gt_arc_imp_mat_ge: assumes gt: "mat_gt_arc m1 m2" and wf: "mat nr nc m1" "mat nr nc m2"
+  shows "mat_ge m1 m2"
+  by (rule mat_geI[OF wf gt_imp_ge[OF mat_comp_allE[OF gt wf]]], auto)  
 
 lemma scalar_prod_left_mono: assumes wf1: "vec nr v1"
   and wf2: "vec nr v2"
@@ -1841,31 +1846,31 @@ lemma mat_arc_pos_zero: assumes n_pos: "n > 0"
 
 lemma mat_gt_arc_compat: assumes ge: "mat_ge m1 m2" and gt: "mat_gt_arc m2 m3" and wf1: "mat nr nc m1" and wf2: "mat nr nc m2" and wf3: "mat nr nc m3" 
   shows "mat_gt_arc m1 m3"
-proof (simp only: mat_comp_all_index[OF wf1 wf3], intro allI impI)
+proof (rule mat_comp_allI[OF wf1 wf3])
   fix i j
   assume i: "i < nc" and j: "j < nr"
-  from ge i j have one: "m1 ! i ! j \<succeq> m2 ! i ! j" using mat_ge_index[OF wf1 wf2] by auto
-  from gt i j have two: "m2 ! i ! j \<succ> m3 ! i ! j" using mat_comp_all_index[OF wf2 wf3] by auto
+  from mat_geE[OF ge wf1 wf2 i j] have one: "m1 ! i ! j \<ge> m2 ! i ! j" .
+  from mat_comp_allE[OF gt wf2 wf3 i j] have two: "m2 ! i ! j \<succ> m3 ! i ! j" .
   from one two show "m1 ! i ! j \<succ> m3 ! i ! j" by (rule compat)
-qed
+qed 
 
 lemma mat_gt_arc_compat2: assumes gt: "mat_gt_arc m1 m2" and ge: "mat_ge m2 m3" and wf1: "mat nr nc m1" and wf2: "mat nr nc m2" and wf3: "mat nr nc m3" 
   shows "mat_gt_arc m1 m3"
-proof (simp only: mat_comp_all_index[OF wf1 wf3], intro allI impI)
+proof (rule mat_comp_allI[OF wf1 wf3])
   fix i j
   assume i: "i < nc" and j: "j < nr"
-  from gt i j have one: "m1 ! i ! j \<succ> m2 ! i ! j" using mat_comp_all_index[OF wf1 wf2] by auto
-  from ge i j have two: "m2 ! i ! j \<succeq> m3 ! i ! j" using mat_ge_index[OF wf2 wf3] by auto
+  from mat_comp_allE[OF gt wf1 wf2 i j] have one: "m1 ! i ! j \<succ> m2 ! i ! j" .
+  from mat_geE[OF ge wf2 wf3 i j] have two: "m2 ! i ! j \<ge> m3 ! i ! j" .
   from one two show "m1 ! i ! j \<succ>  m3 ! i ! j" by (rule compat2)
 qed
 
 lemma mat_gt_arc_trans: assumes gt1: "mat_gt_arc m1 m2" and gt2: "mat_gt_arc m2 m3" and wf1: "mat nr nc m1" and wf2: "mat nr nc m2" and wf3: "mat nr nc m3" 
   shows "mat_gt_arc m1 m3"
-proof (simp only: mat_comp_all_index[OF wf1 wf3], intro allI impI)
+proof (rule mat_comp_allI[OF wf1 wf3])
   fix i j
   assume i: "i < nc" and j: "j < nr"
-  from gt1 i j have one: "m1 ! i ! j \<succ> m2 ! i ! j" using mat_comp_all_index[OF wf1 wf2] by auto
-  from gt2 i j have two: "m2 ! i ! j \<succ> m3 ! i ! j" using mat_comp_all_index[OF wf2 wf3] by auto
+  from mat_comp_allE[OF gt1 wf1 wf2 i j] have one: "m1 ! i ! j \<succ> m2 ! i ! j" .
+  from mat_comp_allE[OF gt2 wf2 wf3 i j] have two: "m2 ! i ! j \<succ> m3 ! i ! j" .
   from one two show "m1 ! i ! j \<succ> m3 ! i ! j" by (rule gt_trans)
 qed
 
@@ -1879,10 +1884,8 @@ lemma mat_gt_arc_plus_mono: assumes gt1: "mat_gt_arc x y"
 proof -
   let ?xz = "mat_plus x z"
   let ?yu = "mat_plus y u"
-  from mat_plus[OF wfx wfz] have wfxz: "mat nr nc ?xz" .
-  from mat_plus[OF wfy wfu] have wfyu: "mat nr nc ?yu" .
-  show ?thesis 
-  proof (simp only: mat_comp_all_index[OF wfxz wfyu], intro allI impI)
+  show ?thesis
+  proof (rule mat_comp_allI)
     fix i j
     assume i: "i < nc" and j: "j < nr"
     show "mat_plus x z ! i ! j \<succ> mat_plus y u ! i ! j"
@@ -1890,11 +1893,10 @@ proof -
         simp only: mat_plus_index[OF wfx wfz i j],
         simp only: mat_plus_index[OF wfy wfu i j],
         rule plus_gt_both_mono)
-      show "x ! i ! j \<succ> y ! i ! j" using gt1 i j mat_comp_all_index[OF wfx wfy] by auto
-    next
-      show "z ! i ! j \<succ> u ! i ! j" using gt2 i j mat_comp_all_index[OF wfz wfu] by auto
+      show "x ! i ! j \<succ> y ! i ! j" using mat_comp_allE[OF gt1 wfx wfy i j] .
+      show "z ! i ! j \<succ> u ! i ! j" using mat_comp_allE[OF gt2 wfz wfu i j] .
     qed
-  qed
+  qed (insert wfx wfy wfz wfu, auto)
 qed
 
 
@@ -1906,10 +1908,8 @@ lemma mat_gt_arc_mult_left_mono: assumes gt1: "mat_gt_arc x y"
 proof -
   let ?xz = "mat_mult nr x z"
   let ?yz = "mat_mult nr y z"
-  from mat_mult[OF wfx wfz] have wfxz: "mat nr ncc ?xz" .
-  from mat_mult[OF wfy wfz] have wfyz: "mat nr ncc ?yz" .
   show ?thesis 
-  proof (simp only: mat_comp_all_index[OF wfxz wfyz], intro allI impI)
+  proof (rule mat_comp_allI)
     fix i j
     assume i: "i < ncc" and j: "j < nr"
     have wfxj: "vec nc (row x j)" using row[OF wfx j] .
@@ -1917,22 +1917,18 @@ proof -
     have wfzi: "vec nc (col z i)" using col[OF wfz i] .
     show "?xz ! i ! j \<succ> ?yz ! i ! j"
     proof (
-        simp only: mat_mult_index[OF wfx wfz j i],
-        simp only: mat_mult_index[OF wfy wfz j i],
+        unfold mat_mult_index[OF wfx wfz j i] mat_mult_index[OF wfy wfz j i],
         rule scalar_prod_left_mono[OF wfxj wfyj wfzi],
-        simp only: vec_comp_all_index[OF wfxj wfyj],
+        unfold vec_comp_all_index[OF wfxj wfyj],
         intro allI impI
       )
       fix k
       assume k: "k < nc"
-      from gt1 mat_comp_all_index[OF wfx wfy, of gt] j k
+      from gt1 mat_comp_all[OF wfx wfy, of gt] j k
       show "row x j ! k \<succ> row y j ! k"
-        by (
-          simp only: row_col[OF wfx j k],
-          simp only: row_col[OF wfy j k],
-          unfold col_def, auto)
+        by (unfold row_col[OF wfx j k] row_col[OF wfy j k] col_def, auto) 
     qed
-  qed
+  qed (insert wfx wfy wfz, auto)
 qed
 
 lemma mat_gt_arc_mult_right_mono: fixes x :: "'a mat" 
@@ -1944,10 +1940,8 @@ lemma mat_gt_arc_mult_right_mono: fixes x :: "'a mat"
 proof -
   let ?xy = "mat_mult nr x y"
   let ?xz = "mat_mult nr x z"
-  from mat_mult[OF wfx wfy] have wfxy: "mat nr ncc ?xy" .
-  from mat_mult[OF wfx wfz] have wfxz: "mat nr ncc ?xz" .
   show ?thesis 
-  proof (simp only: mat_comp_all_index[OF wfxy wfxz], intro allI impI)
+  proof (rule mat_comp_allI)
     fix i j
     assume i: "i < ncc" and j: "j < nr"
     have wfxj: "vec nc (row x j)" using row[OF wfx j] .
@@ -1955,18 +1949,17 @@ proof -
     have wfzi: "vec nc (col z i)" using col[OF wfz i] .
     show "?xy ! i ! j \<succ> ?xz ! i ! j"
     proof (
-        simp only: mat_mult_index[OF wfx wfy j i],
-        simp only: mat_mult_index[OF wfx wfz j i],
+        unfold mat_mult_index[OF wfx wfy j i] mat_mult_index[OF wfx wfz j i],
         rule scalar_prod_right_mono[OF wfxj wfyi wfzi],
-        simp only: vec_comp_all_index[OF wfyi wfzi],
+        unfold vec_comp_all_index[OF wfyi wfzi],
         intro allI impI
       )
       fix k
       assume k: "k < nc"
-      from gt1[unfolded mat_comp_all_index[OF wfy wfz]] i k
+      from gt1[unfolded mat_comp_all[OF wfy wfz]] i k
       show "col y i ! k \<succ> col z i ! k" unfolding col_def by auto
     qed
-  qed
+  qed (insert wfx wfy wfz, auto)
 qed
 
 lemma mat_not_all_ge: assumes n_pos: "n > 0"
@@ -1977,29 +1970,28 @@ lemma mat_not_all_ge: assumes n_pos: "n > 0"
 proof -
   obtain c where c: "c = m1 ! 0 ! 0" by auto
   from a2 have "arc_pos (m2 ! 0 ! 0)" unfolding mat_arc_posI_def .
-  from not_all_ge[OF this, of c] obtain e where e0: "e \<succeq> 0" and ae: "arc_pos e"
-    and nc: "\<not> c \<succeq> m2 ! 0 ! 0 * e" by auto
+  from not_all_ge[OF this, of c] obtain e where e0: "e \<ge> 0" and ae: "arc_pos e"
+    and nc: "\<not> c \<ge> m2 ! 0 ! 0 * e" by auto
   let ?gen = "\<lambda> f. map (\<lambda>i. map (f i) [0..<n]) [0..<n]"
   {
     fix f :: "nat \<Rightarrow> nat \<Rightarrow> 'a" 
     have "mat n n (?gen f)"
       unfolding mat_def by (auto simp: vec_def)    
-  } note gen = this
+  } note gen[simp] = this
   obtain f :: "nat \<Rightarrow> nat \<Rightarrow> 'a" where f: "f = (\<lambda> i j. if i = 0 \<and> j = 0 then e else 0)" by auto
   let ?m = "?gen f"
   have m00: "?m ! 0 ! 0 = e" using n_pos unfolding f by auto
   show ?thesis
   proof (rule exI[of _ ?m], intro conjI, rule gen)
     show "mat_ge ?m (mat0 n n)"
-      unfolding mat_ge_index[OF gen mat0]
-    proof (intro allI impI)
+    proof (rule mat_geI)
       fix i j
       assume i: "i < n" and j: "j < n"
       have m: "?m ! i ! j = f i j" using i j by auto
-      have 0: "mat0 n n ! i ! j = (0 :: 'a)" using mat0_index[OF i j] .
-      show "?m ! i ! j \<succeq> mat0 n n ! i ! j" unfolding m 0
+      have 0: "mat0 n n ! i ! j = (0 :: 'a)" using i j by simp 
+      show "?m ! i ! j \<ge> mat0 n n ! i ! j" unfolding m 0
         unfolding f using e0 ge_refl by auto
-    qed
+    qed auto
   next
     show "mat_arc_pos ?m" 
       unfolding mat_arc_posI_def 
@@ -2030,62 +2022,61 @@ proof -
     also have "... = m2 ! 0 ! 0 * e"
       unfolding scalar_right_zero by simp
     finally have "?mult ! 0 ! 0 = m2 ! 0 ! 0 * e" .
-    with nc c have "\<not> m1 ! 0 ! 0 \<succeq> ?mult ! 0 ! 0" by simp
+    with nc c have "\<not> m1 ! 0 ! 0 \<ge> ?mult ! 0 ! 0" by simp
     thus "\<not> mat_ge m1 ?mult"
-      unfolding mat_ge_index[OF m1 mat_mult[OF m2 gen]] using n_pos
+      unfolding mat_ge_def mat_comp_all[OF m1 mat_mult[OF m2 gen]] using n_pos
       by auto
   qed
 qed
 
 lemma mat0_leastI: assumes wf: "mat nr nc m"
   shows "mat_gt_arc m (mat0 nr nc)"
-proof (simp only: mat_comp_all_index[OF wf mat0], intro allI impI)
+proof (rule mat_comp_allI[OF wf])
   fix i j
   assume i: "i < nc" and j: "j < nr"
-  show "m ! i ! j \<succ> mat0I 0 nr nc ! i ! j"
-    by (simp only: mat0_index[OF i j] zero_leastI)
-qed
+  thus "m ! i ! j \<succ> mat0I 0 nr nc ! i ! j" by (auto simp: zero_leastI)
+qed auto
 
 lemma mat0_leastII: 
   assumes gt: "mat_gt_arc (mat0 nr nc) m"
   and wf: "mat nr nc m"
   shows "m = mat0 nr nc"
-proof (simp only: mat_eq_index[OF wf mat0], intro allI impI)
+proof (rule mat_eqI)
   fix i j
   assume i: "i < nc" and j: "j < nr"
   show "m ! i ! j = mat0 nr nc ! i ! j"
-  proof (simp only: mat0_index[OF i j], rule zero_leastII)
-    show "0 \<succ> m ! i ! j" using i j gt mat_comp_all_index[OF mat0 wf, of gt 0] mat0_index[OF i j, of "0 :: 'a"] by force
+    unfolding mat0_index[OF i j]
+  proof (rule zero_leastII)
+    show "0 \<succ> m ! i ! j" using i j gt mat_comp_all[OF mat0 wf] mat0_index[OF i j] by force
   qed
-qed
+qed (insert wf, auto)
 
 
 lemma mat0_leastIII: assumes wf: "mat nr nc m"
   shows "mat_ge m ((mat0 nr nc) :: 'a mat)"
-proof (simp only: mat_ge_index[OF wf mat0], intro allI impI)
+proof (rule mat_geI[OF wf])
   fix i j
   assume i: "i < nc" and j: "j < nr"
-  show "(m ! i ! j) \<succeq> ((mat0 nr nc :: 'a mat) ! i ! j)"
-    by (simp only: mat0_index[OF i j] zero_leastIII)
-qed
+  show "m ! i ! j \<ge> mat0 nr nc ! i ! j"
+    by (simp add: mat0_index[OF i j] zero_leastIII)
+qed auto
 
 lemma mat1_gt_arc_mat0: "mat_gt_arc (mat1 n) (mat0 n n)"
-proof (simp only: mat_comp_all_index[OF mat1 mat0], intro allI impI)
+proof (rule mat_comp_allI)
   fix i j
   assume i: "i < n" and j: "j < n"
   show "mat1 n ! i ! j \<succ> mat0 n n ! i ! j"
-    by (simp only: mat0_index[OF i j],
-      rule zero_leastI)
-qed
+    by (simp add: mat0_index[OF i j] zero_leastI)
+qed auto
 
 lemma mat_default_gt_arc_mat0: "mat_gt_arc (mat_default n) (mat0 n n)"
-proof (simp only: mat_comp_all_index[OF mat1 mat0], intro allI impI)
+proof (rule mat_comp_allI)
   fix i j
   assume i: "i < n" and j: "j < n"
   show "mat_default n ! i ! j \<succ> mat0 n n ! i ! j"
     by (simp only: mat0_index[OF i j],
       rule zero_leastI)
-qed
+qed auto
 end 
 
 context SN_both_mono_ordered_semiring_1
@@ -2101,11 +2092,10 @@ proof (rule ccontr)
   proof
     fix i
     from steps have wf1: "mat n n (f i)" and wf2: "mat n n (f (Suc i))" and gt: "mat_gt_arc (f i) (f (Suc i))" by auto
-    show "f i ! 0 ! 0 \<succ>  f (Suc i) ! 0 ! 0" using mat_comp_all_index[OF wf1 wf2, of gt] mat0_index[OF n_pos n_pos, of 0] gt n_pos by force
+    show "f i ! 0 ! 0 \<succ>  f (Suc i) ! 0 ! 0" using mat_comp_allE[OF gt wf1 wf2] mat0_index[OF n_pos n_pos, of 0] n_pos by force
   qed
   from pos gt SN show False unfolding SN_defs by force
 qed
-
 
 
 lemma mat_arc_pos_plus: assumes n_pos: "n > 0" 
@@ -2143,9 +2133,9 @@ proof -
 qed
 
 lemma mat_arc_pos_mat_default: assumes n_pos: "n > 0" shows "mat_arc_pos (mat_default n)"
-unfolding mat1I_def mat_arc_posI_def 
-using n_pos
-by (auto simp: vec1I_def arc_pos_default)
+  unfolding mat1I_def mat_arc_posI_def 
+  using n_pos
+  by (auto simp: vec1I_def arc_pos_default)
 end
 
 
@@ -2172,7 +2162,7 @@ proof -
     fix m1 m2
     assume ass: "mat n n m1 \<and> mat n n m2 \<and> (m1,m2) \<in> set m12s"
     hence wf1: "mat n n m1" and wf2: "mat n n m2" and m1m2: "(m1,m2) \<in> set m12s" by auto
-    from orient[OF ass, unfolded mat_gt_index[OF wf1 wf2 sd_n]] 
+    from orient[OF ass, unfolded mat_gt[OF wf1 wf2 sd_n]] 
     obtain i j where ge: "mat_ge m1 m2" and i: "i < sd" and j: "j < sd" and weak_gt: "weak_gt (m1 ! i ! j) (m2 ! i ! j)" (is "weak_gt ?x ?y") by auto
     from wf1 i j sd_n have m1ij: "m1 ! i \<in> set m1 \<and> m1 ! i ! j \<in> set (m1 ! i)" unfolding mat_def  by (auto simp: vec_def)
     from wf2 i j sd_n have m2ij: "m2 ! i \<in> set m2 \<and> m2 ! i ! j \<in> set (m2 ! i)" unfolding mat_def  by (auto simp: vec_def)
@@ -2180,7 +2170,7 @@ proof -
     have y: "?y \<in> set ?m2y" by (auto, rule bexI[OF _ m1m2], rule bexI[of _ "m2 ! i"], auto simp: m2ij)
     from x y have "(?x,?y) \<in> set ?pairs" by force
     with weak_gt have gt: "(?x,?y) \<in> set ?strict" by simp
-    show "mat_gtI gt sd m1 m2" unfolding mat_gt_index[OF wf1 wf2 sd_n]
+    show "mat_gtI gt sd m1 m2" unfolding mat_gt[OF wf1 wf2 sd_n]
       by (intro exI conjI, rule ge, rule i, rule j, rule orient2[OF gt])
   qed (rule order)
 qed
@@ -2208,11 +2198,12 @@ proof -
     fix m1 m2
     assume ass: "mat n n m1 \<and> mat n n m2 \<and> (m1,m2) \<in> set m12s"
     hence wf1: "mat n n m1" and wf2: "mat n n m2" and m1m2: "(m1,m2) \<in> set m12s" by auto
-    show "mat_comp_all gt  m1 m2" unfolding mat_comp_all_index[OF wf1 wf2]
-    proof (intro allI impI)
+    show "mat_comp_all gt  m1 m2" 
+    proof (rule mat_comp_allI[OF wf1 wf2])
       fix i j
       assume i: "i < n" and j: "j < n"
-      with orient[OF ass, unfolded mat_comp_all_index[OF wf1 wf2]] have weak_gt: "weak_gt (m1 ! i ! j) (m2 ! i ! j)" (is "weak_gt ?x ?y") by auto  
+      from mat_comp_allE[OF orient[OF ass] wf1 wf2 this]
+      have weak_gt: "weak_gt (m1 ! i ! j) (m2 ! i ! j)" (is "weak_gt ?x ?y") by auto  
       from wf1 i j have m1ij: "m1 ! i \<in> set m1 \<and> m1 ! i ! j \<in> set (m1 ! i)" unfolding mat_def  by (auto simp: vec_def)
       from wf2 i j have m2ij: "m2 ! i \<in> set m2 \<and> m2 ! i ! j \<in> set (m2 ! i)" unfolding mat_def  by (auto simp: vec_def)
       have x: "?x \<in> set ?m1x" by (simp, rule bexI[OF _ m1m2], rule bexI[of _ "m1 ! i"], auto simp: m1ij)
@@ -2224,5 +2215,48 @@ proof -
   qed
 qed
 end
+
+subsection {* Connection to ordered semirings *}
+
+definition mat_ordered_semiring :: "nat \<Rightarrow> nat \<Rightarrow> ('a :: ordered_semiring_1 \<Rightarrow> 'a \<Rightarrow> bool) \<Rightarrow> 'b \<Rightarrow> ('a mat,'b) ordered_semiring_scheme" where
+  "mat_ordered_semiring n sd gt b \<equiv> mat_ring n \<lparr>
+    ordered_semiring.geq = mat_ge,
+    gt = mat_gtI gt sd,
+    max = mat_max,
+    \<dots> = b\<rparr>"
+
+lemma (in one_mono_ordered_semiring_1) mat_ordered_semiring: assumes sd_n: "sd \<le> n" 
+  shows "ordered_semiring 
+    (mat_ordered_semiring n sd op \<succ> b :: ('a mat,'b) ordered_semiring_scheme)" 
+  (is "ordered_semiring ?R")
+proof -
+  interpret semiring ?R unfolding mat_ordered_semiring_def by (rule mat_semiring)
+  show ?thesis 
+    by (unfold_locales, unfold mat_ring_def mat_ordered_semiring_def ordered_semiring_record_simps,
+      auto intro: mat_max_comm mat_gt_compat[OF sd_n] mat_gt_compat2[OF sd_n] mat_ge_trans
+      mat_plus_left_mono mat_mult_left_mono mat_mult_right_mono mat_ge_refl mat_gt_imp_mat_ge
+      mat1_ge_mat0 mat_max_mono mat_max_ge mat_max_id)
+qed
+
+definition mat_both_ordered_semiring :: "nat \<Rightarrow> ('a :: ordered_semiring_1 \<Rightarrow> 'a \<Rightarrow> bool) \<Rightarrow> 'b \<Rightarrow> ('a mat,'b) ordered_semiring_scheme" where
+  "mat_both_ordered_semiring n gt b \<equiv> mat_ring n \<lparr>
+    ordered_semiring.geq = mat_ge,
+    gt = mat_comp_all gt,
+    max = mat_max,
+    \<dots> = b\<rparr>"
+
+lemma (in both_mono_ordered_semiring_1) mat_both_ordered_semiring: assumes n: "n > 0" 
+  shows "ordered_semiring 
+    (mat_both_ordered_semiring n op \<succ> b :: ('a mat,'b) ordered_semiring_scheme)" 
+  (is "ordered_semiring ?R")
+proof -
+  interpret semiring ?R unfolding mat_both_ordered_semiring_def by (rule mat_semiring)
+  show ?thesis 
+    by (unfold_locales, unfold mat_ring_def mat_both_ordered_semiring_def ordered_semiring_record_simps,
+      auto intro: mat_max_comm mat_ge_trans
+      mat_plus_left_mono mat_mult_left_mono mat_mult_right_mono mat_ge_refl
+      mat1_ge_mat0 mat_max_mono mat_max_ge mat_max_id mat_gt_arc_trans mat_gt_arc_imp_mat_ge
+      mat_gt_arc_compat mat_gt_arc_compat2)
+qed
 
 end
