thy_lib/isabelle_afp/Containers/Collection_Eq.thy
@@ -1,0 +1,127 @@
+(*  Title:      Containers/Collection_Eq.thy
+    Author:     Andreas Lochbihler, KIT
+                René Thiemann, UIBK *)
+theory Collection_Eq imports
+  Auxiliary
+  Containers_Generator
+begin
+
+section {* A type class for optional equality testing *}
+
+class ceq =
+  fixes ceq :: "('a \<Rightarrow> 'a \<Rightarrow> bool) option"
+  assumes ceq: "ceq = Some eq \<Longrightarrow> eq = op ="
+begin
+
+lemma ID_ceq: "ID ceq = Some eq \<Longrightarrow> eq = op ="
+unfolding ID_def id_apply by(rule ceq)
+
+abbreviation ceq' :: "'a \<Rightarrow> 'a \<Rightarrow> bool" where "ceq' \<equiv> the (ID ceq)"
+
+end
+
+syntax "_CEQ" :: "type => logic"  ("(1CEQ/(1'(_')))")
+
+parse_translation {*
+let
+  fun ceq_tr [ty] =
+     (Syntax.const @{syntax_const "_constrain"} $ Syntax.const @{const_syntax "ceq"} $
+       (Syntax.const @{type_syntax option} $ 
+         (Syntax.const @{type_syntax fun} $ ty $ 
+           (Syntax.const @{type_syntax fun} $ ty $ Syntax.const @{type_syntax bool}))))
+    | ceq_tr ts = raise TERM ("ceq_tr", ts);
+in [(@{syntax_const "_CEQ"}, K ceq_tr)] end
+*}
+
+typed_print_translation {*
+let
+  fun ceq_tr' ctxt
+    (Type (@{type_name option}, [Type (@{type_name fun}, [T, _])])) ts =
+    Term.list_comb (Syntax.const @{syntax_const "_CEQ"} $ Syntax_Phases.term_of_typ ctxt T, ts)
+  | ceq_tr' _ _ _ = raise Match;
+in [(@{const_syntax ceq}, ceq_tr')]
+end
+*}
+
+definition is_ceq :: "'a :: ceq itself \<Rightarrow> bool"
+where "is_ceq _ \<longleftrightarrow> ID CEQ('a) \<noteq> None"
+
+subsection {* Generator for the @{class ceq}-class *}
+
+text {*
+This generator registers itself at the derive-manager for the class @{class ceq}.
+To be more precise, one can choose whether one wants to take @{term "op ="} as function
+for @{term ceq} by passing "eq" as parameter, 
+whether equality should not be supported by passing "no" as parameter,
+or whether an own definition for equality should be derived by not passing
+any parameters. The last possibility only works for datatypes.
+
+\begin{itemize}
+\item \texttt{instantiation type :: (type,\ldots,type) (eq) ceq}
+\item \texttt{instantiation type :: (type,\ldots,type) (no) ceq}
+\item \texttt{instantiation datatype :: (ceq,\ldots,ceq) ceq}
+\end{itemize}
+
+If the parameter "no" is not used, then the corresponding
+@{term is_ceq}-theorem is also automatically generated and attributed with 
+\texttt{[simp, code-post]}.
+*}
+
+
+text {*
+This generator can be used for arbitrary types, not just datatypes. 
+*}
+
+ML_file "ceq_generator.ML"
+
+setup {*
+  Ceq_Generator.setup
+*}
+
+subsection {* Type class instances for HOL types *}
+
+derive (eq) ceq unit
+lemma [code]: "CEQ(unit) = Some (\<lambda>_ _. True)"
+  unfolding ceq_unit_def by (simp, intro ext, auto)
+derive (eq) ceq bool
+derive (eq) ceq nat
+derive (eq) ceq int
+derive (eq) ceq Enum.finite_1
+derive (eq) ceq Enum.finite_2
+derive (eq) ceq Enum.finite_3
+derive (eq) ceq Enum.finite_4
+derive (eq) ceq Enum.finite_5
+derive (eq) ceq integer
+derive (eq) ceq natural
+derive (eq) ceq nibble
+derive (eq) ceq char
+derive (eq) ceq String.literal
+derive ceq sum
+derive ceq prod
+derive ceq list
+derive ceq option
+derive (no) ceq "fun"
+
+lemma is_ceq_fun [simp]: "\<not> is_ceq TYPE('a \<Rightarrow> 'b)"
+  by(simp add: is_ceq_def ceq_fun_def ID_None) 
+
+definition set_eq :: "'a set \<Rightarrow> 'a set \<Rightarrow> bool" 
+where [code del]: "set_eq = op ="
+
+lemma set_eq_code:
+  shows [code]: "set_eq A B \<longleftrightarrow> A \<subseteq> B \<and> B \<subseteq> A"
+  and [code_unfold]: "op = = set_eq"
+unfolding set_eq_def by blast+
+
+instantiation set :: (ceq) ceq begin
+definition "CEQ('a set) = (case ID CEQ('a) of None \<Rightarrow> None | Some _ \<Rightarrow> Some set_eq)"
+instance by(intro_classes)(simp add: ceq_set_def set_eq_def split: option.splits)
+end
+
+lemma is_ceq_set [simp, code_post]: "is_ceq TYPE('a set) \<longleftrightarrow> is_ceq TYPE('a :: ceq)"
+by(simp add: is_ceq_def ceq_set_def ID_None ID_Some split: option.split)
+
+lemma ID_ceq_set_not_None_iff [simp]: "ID CEQ('a set) \<noteq> None \<longleftrightarrow> ID CEQ('a :: ceq) \<noteq> None"
+by(simp add: ceq_set_def ID_def split: option.splits)
+
+end
