thy_lib/isabelle_afp/Containers/ITP-2013/Benchmark_LC.thy
@@ -1,0 +1,12 @@
+theory Benchmark_LC imports
+  Benchmark_Comparison
+  "../Set_Impl"
+  "~~/src/HOL/Library/Code_Target_Nat"
+begin
+
+notepad begin
+  have "complete 200 (12345, 67889) = (48, 50)"
+    by eval
+end
+
+end
