thy_lib/isabelle_afp/Containers/ITP-2013/Benchmark_Set_Default.thy
@@ -1,0 +1,22 @@
+theory Benchmark_Set_Default 
+imports
+  Benchmark_Set
+  "~~/src/HOL/Library/Code_Target_Nat"
+begin
+
+text {* Implement set equality for all combinations of @{term "List.set"} and @{term "List.coset"} *}
+lemma [code]: "equal_class.equal A B \<longleftrightarrow> Cardinality.eq_set A B" 
+ by(simp add: equal_eq)
+
+ML_val {*
+  val seed = (Code_Numeral.natural_of_integer 12345, Code_Numeral.natural_of_integer 67889);
+  val n = @{code nat_of_integer} 30;
+  val m = @{code nat_of_integer} 40;
+  val c = @{code complete} n m seed;
+*}
+
+notepad begin
+  have "complete 30 40 (12345, 67889) = (30, 4294967296)" by eval
+end
+
+end
