thy_lib/isabelle_afp/Containers/Mapping_Impl.thy
@@ -1,0 +1,273 @@
+(*  Title:      Containers/Mapping_Impl.thy
+    Author:     Andreas Lochbihler, KIT
+                René Thiemann, UIBK *)
+
+theory Mapping_Impl imports 
+  RBT_Mapping2
+  AssocList
+  "~~/src/HOL/Library/Mapping"
+  Set_Impl
+  Containers_Generator
+begin
+
+section {* Different implementations of maps *}
+
+code_identifier
+  code_module Mapping \<rightharpoonup> (SML) Mapping_Impl
+| code_module Mapping_Impl \<rightharpoonup> (SML) Mapping_Impl
+
+subsection {* Map implementations *}
+
+definition Assoc_List_Mapping :: "('a, 'b) alist \<Rightarrow> ('a, 'b) mapping"
+where [simp]: "Assoc_List_Mapping al = Mapping.Mapping (DAList.lookup al)"
+
+definition RBT_Mapping :: "('a :: corder, 'b) mapping_rbt \<Rightarrow> ('a, 'b) mapping"
+where [simp]: "RBT_Mapping t = Mapping.Mapping (RBT_Mapping2.lookup t)"
+
+code_datatype Assoc_List_Mapping RBT_Mapping Mapping
+
+subsection {* Map operations *}
+
+lemma [code, code del]: "Mapping.lookup = Mapping.lookup" ..
+
+lemma lookup_Mapping_code [code]:
+  "Mapping.lookup (Assoc_List_Mapping al) = DAList.lookup al"
+  "Mapping.lookup (RBT_Mapping t) = RBT_Mapping2.lookup t"
+by(simp_all)(transfer, rule)+
+
+lemma [code, code del]: "Mapping.is_empty = Mapping.is_empty" ..
+
+context
+begin
+interpretation lifting_syntax .
+
+lemma is_empty_transfer [transfer_rule]:
+  "(pcr_mapping op = op = ===> op =) (\<lambda>m. m = empty) Mapping.is_empty"
+unfolding mapping.pcr_cr_eq
+apply(rule fun_relI)
+apply(case_tac y)
+apply(simp add: Mapping.is_empty_def cr_mapping_def Mapping_inverse Mapping.keys.rep_eq)
+done
+
+end
+
+lemma is_empty_Mapping [code]:
+  fixes t :: "('a :: corder, 'b) mapping_rbt" shows
+  "Mapping.is_empty (Assoc_List_Mapping al) \<longleftrightarrow> al = DAList.empty"
+  "Mapping.is_empty (RBT_Mapping t) \<longleftrightarrow>
+  (case ID CORDER('a) of None \<Rightarrow> Code.abort (STR ''is_empty RBT_Mapping: corder = None'') (\<lambda>_. Mapping.is_empty (RBT_Mapping t))
+                     | Some _ \<Rightarrow> RBT_Mapping2.is_empty t)"
+apply(simp_all split: option.split)
+ apply(transfer, case_tac al, simp_all)
+apply(transfer, simp)
+done
+
+lemma [code, code del]: "Mapping.update = Mapping.update" ..
+
+lemma update_Mapping [code]:
+  fixes t :: "('a :: corder, 'b) mapping_rbt" shows
+  "Mapping.update k v (Mapping m) = Mapping (m(k \<mapsto> v))"
+  "Mapping.update k v (Assoc_List_Mapping al) = Assoc_List_Mapping (DAList.update k v al)"
+  "Mapping.update k v (RBT_Mapping t) =
+  (case ID CORDER('a) of None \<Rightarrow> Code.abort (STR ''update RBT_Mapping: corder = None'') (\<lambda>_. Mapping.update k v (RBT_Mapping t))
+                     | Some _ \<Rightarrow> RBT_Mapping (RBT_Mapping2.insert k v t))" (is ?RBT)
+by(simp_all split: option.split)(transfer, simp)+
+
+lemma [code, code del]: "Mapping.delete = Mapping.delete" ..
+
+lemma delete_Mapping [code]:
+  fixes t :: "('a :: corder, 'b) mapping_rbt" shows
+  "Mapping.delete k (Mapping m) = Mapping (m(k := None))"
+  "Mapping.delete k (Assoc_List_Mapping al) = Assoc_List_Mapping (AssocList.delete k al)"
+  "Mapping.delete k (RBT_Mapping t) = 
+  (case ID CORDER('a) of None \<Rightarrow> Code.abort (STR ''delete RBT_Mapping: corder = None'') (\<lambda>_. Mapping.delete k (RBT_Mapping t))
+                     | Some _ \<Rightarrow> RBT_Mapping (RBT_Mapping2.delete k t))"
+by(simp_all split: option.split)(transfer, simp)+
+
+lemma [code, code del]: "Mapping.keys = Mapping.keys" ..
+
+theorem (in ord) rbt_lookup_map_const: "rbt_lookup (RBT_Impl.map (\<lambda>_. f) t) = Option.map f \<circ> rbt_lookup t"
+by(induct t)(simp_all add: fun_eq_iff)
+
+lemma keys_Mapping [code]:
+  fixes t :: "('a :: corder, 'b) mapping_rbt" shows
+  "Mapping.keys (Mapping m) = Collect (\<lambda>k. m k \<noteq> None)" (is "?Mapping")
+  "Mapping.keys (Assoc_List_Mapping al) = AssocList.keys al" (is "?Assoc_List")
+  "Mapping.keys (RBT_Mapping t) = RBT_set (RBT_Mapping2.map (\<lambda>_ _. ()) t)" (is "?RBT")
+proof -
+  show ?Mapping by transfer auto
+  show ?Assoc_List by simp(transfer, auto intro: rev_image_eqI)
+  show ?RBT
+    by(simp add: RBT_set_def)(transfer, auto simp add: ord.rbt_lookup_map_const o_def)
+qed
+
+lemma [code, code del]: "Mapping.size = Mapping.size" ..
+
+context
+begin
+interpretation lifting_syntax .
+
+lemma Mapping_size_transfer [transfer_rule]:
+  "(pcr_mapping op = op = ===> op =) (card \<circ> dom) Mapping.size"
+apply(rule fun_relI)
+apply(case_tac y)
+apply(simp add: Mapping.size_def Mapping.keys.rep_eq Mapping_inverse mapping.pcr_cr_eq cr_mapping_def)
+done
+
+end
+
+lemma size_Mapping [code]:
+  fixes t :: "('a :: corder, 'b) mapping_rbt" shows
+  "Mapping.size (Assoc_List_Mapping al) = size al"
+  "Mapping.size (RBT_Mapping t) =
+  (case ID CORDER('a) of None \<Rightarrow> Code.abort (STR ''size RBT_Mapping: corder = None'') (\<lambda>_. Mapping.size (RBT_Mapping t))
+                     | Some _ \<Rightarrow> length (RBT_Mapping2.entries t))"
+apply(simp_all split: option.split)
+apply(transfer, simp add: dom_map_of_conv_image_fst set_map[symmetric] distinct_card del: set_map)
+apply transfer
+apply(clarsimp simp add: size_eq_card_dom_lookup)
+apply(simp add: linorder.rbt_lookup_keys[OF ID_corder] ord.is_rbt_rbt_sorted RBT_Impl.keys_def distinct_card linorder.distinct_entries[OF ID_corder] del: set_map)
+apply(subst distinct_card)
+apply(rule linorder.distinct_entries[OF ID_corder], assumption)
+apply(simp_all add: ord.is_rbt_rbt_sorted)
+done
+
+
+lemma [code, code del]: "Mapping.tabulate = Mapping.tabulate" ..
+
+lemma tabulate_Mapping [code]:
+  "Mapping.tabulate xs f = fold (\<lambda>k m. Mapping.update k (f k) m) xs Mapping.empty"
+apply(rule sym)
+apply transfer
+apply(unfold tabulate_alt_def)
+apply(induct_tac xs rule: rev_induct)
+apply(auto simp add: fun_eq_iff restrict_map_def)
+done
+
+datatype mapping_impl = Mapping_IMPL
+declare mapping_impl.eq.simps [code del]
+
+definition mapping_Choose :: mapping_impl where [simp]: "mapping_Choose = Mapping_IMPL"
+definition mapping_Assoc_List :: mapping_impl where [simp]: "mapping_Assoc_List = Mapping_IMPL"
+definition mapping_RBT :: mapping_impl where [simp]: "mapping_RBT = Mapping_IMPL"
+definition mapping_Mapping :: mapping_impl where [simp]: "mapping_Mapping = Mapping_IMPL"
+
+code_datatype mapping_Choose mapping_Assoc_List mapping_RBT mapping_Mapping
+
+definition mapping_empty_choose :: "('a, 'b) mapping" 
+where [simp]: "mapping_empty_choose = Mapping.empty"
+
+lemma mapping_empty_choose_code [code]:
+  "(mapping_empty_choose :: ('a :: corder, 'b) mapping) =
+   (case ID CORDER('a) of Some _  \<Rightarrow> RBT_Mapping RBT_Mapping2.empty
+    | None \<Rightarrow> Assoc_List_Mapping DAList.empty)"
+by(auto split: option.split simp add: DAList.lookup_empty[abs_def] Mapping.empty_def)
+
+definition mapping_impl_choose2 :: "mapping_impl \<Rightarrow> mapping_impl \<Rightarrow> mapping_impl"
+where [simp]: "mapping_impl_choose2 = (\<lambda>_ _. Mapping_IMPL)"
+
+lemma mapping_impl_choose2_code [code]:
+  "mapping_impl_choose2 x y = mapping_Choose"
+  "mapping_impl_choose2 mapping_Mapping mapping_Mapping = mapping_Mapping"
+  "mapping_impl_choose2 mapping_Assoc_List mapping_Assoc_List = mapping_Assoc_List"
+  "mapping_impl_choose2 mapping_RBT mapping_RBT = mapping_RBT"
+by(simp_all)
+
+definition mapping_empty :: "mapping_impl \<Rightarrow> ('a, 'b) mapping"
+where [simp]: "mapping_empty = (\<lambda>_. Mapping.empty)"
+
+lemma mapping_empty_code [code]:
+  "mapping_empty mapping_Choose = mapping_empty_choose"
+  "mapping_empty mapping_Mapping = Mapping (\<lambda>_. None)"
+  "mapping_empty mapping_Assoc_List = Assoc_List_Mapping DAList.empty"
+  "mapping_empty mapping_RBT = RBT_Mapping RBT_Mapping2.empty"
+by(simp_all add: Mapping.empty_def DAList.lookup_empty[abs_def])
+
+subsection {* Type classes *}
+
+class mapping_impl = 
+  fixes mapping_impl :: "('a, mapping_impl) phantom"
+
+syntax (input)
+  "_MAPPING_IMPL" :: "type => logic"  ("(1MAPPING'_IMPL/(1'(_')))")
+
+parse_translation {*
+let
+  fun mapping_impl_tr [ty] =
+     (Syntax.const @{syntax_const "_constrain"} $ Syntax.const @{const_syntax "mapping_impl"} $
+       (Syntax.const @{type_syntax phantom} $ ty $ Syntax.const @{type_syntax mapping_impl}))
+    | mapping_impl_tr ts = raise TERM ("mapping_impl_tr", ts);
+in [(@{syntax_const "_MAPPING_IMPL"}, K mapping_impl_tr)] end
+*}
+
+lemma [code, code del]: "Mapping.empty = Mapping.empty" ..
+
+lemma Mapping_empty_code [code, code_unfold]: 
+  "(Mapping.empty :: ('a :: mapping_impl, 'b) mapping) =
+   mapping_empty (of_phantom MAPPING_IMPL('a))"
+by simp
+
+subsection {* Generator for the @{class mapping_impl}-class *}
+
+text {*
+This generator registers itself at the derive-manager for the classes @{class mapping_impl}.
+Here, one can choose
+the desired implementation via the parameter. 
+
+\begin{itemize}
+\item \texttt{instantiation type :: (type,\ldots,type) (rbt,assoclist,mapping,choose, or arbitrary constant name) mapping-impl}
+\end{itemize}
+*}
+
+
+text {*
+This generator can be used for arbitrary types, not just datatypes. 
+*}
+
+ML_file "mapping_impl_generator.ML" 
+
+setup {*
+  Mapping_Impl_Generator.setup
+*}
+
+derive (assoclist) mapping_impl unit
+derive (assoclist) mapping_impl bool
+derive (rbt) mapping_impl nat
+derive (mapping_RBT) mapping_impl int (* shows usage of constant names *)
+derive (assoclist) mapping_impl Enum.finite_1
+derive (assoclist) mapping_impl Enum.finite_2
+derive (assoclist) mapping_impl Enum.finite_3
+derive (rbt) mapping_impl integer
+derive (rbt) mapping_impl natural
+derive (assoclist) mapping_impl nibble
+derive (rbt) mapping_impl char
+
+instantiation sum :: (mapping_impl, mapping_impl) mapping_impl begin
+definition "MAPPING_IMPL('a + 'b) = Phantom('a + 'b) 
+  (mapping_impl_choose2 (of_phantom MAPPING_IMPL('a)) (of_phantom MAPPING_IMPL('b)))"
+instance ..
+end
+
+instantiation prod :: (mapping_impl, mapping_impl) mapping_impl begin
+definition "MAPPING_IMPL('a * 'b) = Phantom('a * 'b) 
+  (mapping_impl_choose2 (of_phantom MAPPING_IMPL('a)) (of_phantom MAPPING_IMPL('b)))"
+instance ..
+end
+
+derive (choose) mapping_impl list
+derive (rbt) mapping_impl String.literal
+
+instantiation option :: (mapping_impl) mapping_impl begin
+definition "MAPPING_IMPL('a option) = Phantom('a option) (of_phantom MAPPING_IMPL('a))"
+instance ..
+end
+
+derive (choose) mapping_impl set
+
+instantiation phantom :: (type, mapping_impl) mapping_impl begin
+definition "MAPPING_IMPL(('a, 'b) phantom) = Phantom (('a, 'b) phantom) 
+  (of_phantom MAPPING_IMPL('b))"
+instance ..
+end
+
+end
