thy_lib/isabelle_afp/Dijkstra_Shortest_Path/Weight.thy
@@ -58,7 +58,10 @@ instance int :: weight ..
 instance rat :: weight ..
 instance real :: weight ..
 
-class top_weight = top + weight +
+term top
+
+
+class top_weight = order_top + weight +
   assumes inf_add_right[simp]: "a + top = top"
 begin
 
